[Checkpoint] Handle crash oracle handling in Language.v Saving in case I need to revert.

src/Framework/Layer/Language.v
@@ -1,4 +1,4 @@
-Require Import Primitives Layer.Core.
+Require Import Primitives Layer.Core Lia.
 Import ListNotations.
 
 Set Implicit Arguments.
@@ -50,9 +50,9 @@ Section Language.
              
   | ExecBindCrash :
       forall T T' (p1: prog' T) (p2: T -> prog' T')
-        u o1 o2 d1 d1',
+        u o1 d1 d1',
         exec' u o1 d1 p1 (Crashed d1') ->
-        exec' u (o1++o2) d1 (Bind p1 p2) (Crashed d1').
+        exec' u o1 d1 (Bind p1 p2) (Crashed d1').
 
   Inductive recovery_exec' :
     forall T, user -> list oracle' -> state' -> list (state' -> state') -> prog' T -> prog' unit -> @Recovery_Result state' T -> Prop :=
@@ -93,6 +93,19 @@ Notation "x <-| p1 ; p2" := (Bind (Op _ p1) (fun x => p2))(right associativity, 
 
 
  (** Facts **)
+
+ Lemma exec_empty_oracle:
+      forall O (L: Language O) T (p: prog L T) u s s',
+      ~ exec L u [] s p s'.
+      induction p; unfold not; intros.
+      inversion H; cleanup.
+      inversion H; cleanup.
+      inversion H0; cleanup.
+      apply app_eq_nil in H1; cleanup.
+      simpl in *; eauto.
+      eapply IHp; eauto.
+      eapply IHp; eauto.
+  Qed.
 
 Lemma exec_finished_deterministic_prefix:
   forall O (L: Language O) T (p: prog L T) u o1 o2 o3 o4 s s1 s2 r1 r2,
@@ -147,8 +160,7 @@ Proof.
   - rewrite <- app_assoc in H12; eauto.
     eapply exec_finished_deterministic_prefix in H8; eauto; cleanup; eauto.
     
-  - rewrite <- app_assoc in H12; eauto.
-    clear H1; eapply finished_not_crashed_oracle_prefix in H8; eauto.
+  - rewrite <- app_assoc in H17; eauto.
     Unshelve.
     all: eauto.  
 Qed.
@@ -222,3 +234,330 @@ Proof.
   all: eauto.
 Qed.
 
+Definition minimal_oracle {O} {L: Language O} {T} (p: L.(prog) T) u s o om :=
+forall s',
+      exec L u o s p s' ->
+      exists o',
+      o = om ++ o' /\
+      exec L u om s p s' /\
+      (forall n r, 
+      n < length om ->
+      ~exec L u (firstn n om) s p r).
+
+
+Lemma minimal_oracle_finished_same :
+forall O (L: Language O) T (p: prog L T) o u s s' r,
+exec L u o s p (Finished s' r) ->
+minimal_oracle p u s o o.
+Proof.
+  induction p; simpl; intros.
+  {
+    unfold minimal_oracle; intros.
+    eapply exec_deterministic_wrt_oracle in H; eauto; cleanup.
+    exists nil; simpl; intuition eauto.
+    rewrite app_nil_r; eauto.
+    inversion H0; cleanup.
+    simpl in *.
+    destruct n; try lia.
+    simpl in *; eapply exec_empty_oracle; eauto.
+  }
+  {
+    unfold minimal_oracle; intros.
+    eapply exec_deterministic_wrt_oracle in H; eauto; cleanup.
+    exists nil; simpl; intuition eauto.
+    rewrite app_nil_r; eauto.
+    inversion H0; cleanup.
+    simpl in *.
+    destruct n; try lia.
+    simpl in *; eapply exec_empty_oracle; eauto.
+  }
+  { 
+    unfold minimal_oracle in *; intros.
+    eapply exec_deterministic_wrt_oracle in H0; eauto; cleanup.
+    inversion H1; cleanup; eauto.
+    eapply_fresh H in H10; eauto.
+    eapply_fresh IHp in H7; eauto.
+    logic_clean.
+    exists nil; intuition eauto.
+    rewrite app_nil_r; eauto.
+
+    rewrite app_length in *.
+    destruct (PeanoNat.Nat.eq_dec n (length o1)).
+
+    rewrite firstn_app_l in H9; eauto.
+    rewrite firstn_oob in H9; eauto.
+    inversion H9; subst; sigT_eq.
+    eapply exec_finished_deterministic_prefix in H7; eauto.
+    logic_clean.
+    
+    assert (length o0 = length o0 + length o3). {
+      rewrite H7 at 1.
+      rewrite app_length; eauto.
+    }
+    assert (length o3 = 0). { lia. }
+    apply length_zero_iff_nil in H14; subst;
+    eapply exec_empty_oracle; eauto.
+    eapply finished_not_crashed_oracle_prefix. 
+    apply H7.
+    2: eauto.
+    eauto.
+    all: try lia.
+    
+    apply PeanoNat.Nat.lt_gt_cases in n0.
+    destruct n0.
+    {
+      rewrite firstn_app_l in H9; eauto.
+      inversion H9; subst; sigT_eq.
+      destruct o3.
+      eapply exec_empty_oracle; eauto.
+      assert (exists m, o0 = firstn m o1 /\ m < length o1). {
+      rewrite <- firstn_skipn with (n:= length o0) in H12.
+      eapply app_split_length_eq_l in H12. 
+      logic_clean; subst.
+      rewrite firstn_firstn in H12.
+      eexists; eauto.
+      split; eauto.
+      eapply PeanoNat.Nat.min_lt_iff; eauto.
+      rewrite firstn_skipn in H12.
+      rewrite <- H12.
+      rewrite firstn_app2; eauto.
+    }
+    logic_clean; subst.
+    eapply H4; eauto.
+    eapply finished_not_crashed_oracle_prefix. 
+    apply H7.
+    2: eauto.
+    rewrite app_nil_r; eauto.
+    erewrite firstn_skipn with (l:= o1); eauto.
+    lia.
+    }
+    {
+      rewrite firstn_app_le in H9.
+    inversion H9; subst; sigT_eq.
+    eapply exec_finished_deterministic_prefix in H7; eauto.
+    logic_clean; subst; clear_lists; subst.
+    eapply H6; eauto.
+    lia.
+    eapply finished_not_crashed_oracle_prefix in H7; eauto.
+    rewrite <- app_assoc; eauto.
+    lia.
+    }
+  }
+  Unshelve.
+  all: eauto.
+Qed.
+
+
+  Lemma minimal_oracle_exists :
+forall O (L: Language O) T (p: prog L T) u o s r,
+exec L u o s p r ->
+exists om, minimal_oracle p u s o om.
+Proof.
+  induction p; simpl; intros.
+  {
+    unfold minimal_oracle; intros.
+    eexists; intros.
+    inversion H; cleanup.
+    exists nil; intuition eauto.
+    rewrite app_nil_r; eauto.
+    simpl in *.
+    destruct n; try lia.
+    simpl in *; eapply exec_empty_oracle; eauto.
+    
+    exists nil; intuition eauto.
+    simpl in *.
+    destruct n; try lia.
+    simpl in *; eapply exec_empty_oracle; eauto.
+  }
+  {
+    unfold minimal_oracle; intros.
+    eexists; intros.
+    inversion H; cleanup.
+    exists nil; intuition eauto.
+    rewrite app_nil_r; eauto.
+    simpl in *.
+    destruct n; try lia.
+    simpl in *; eapply exec_empty_oracle; eauto.
+    
+    exists nil; intuition eauto.
+    simpl in *.
+    destruct n; try lia.
+    simpl in *; eapply exec_empty_oracle; eauto.
+  }
+  {
+    
+    inversion H0; cleanup; eauto.
+    edestruct IHp; eauto.
+    eapply_fresh minimal_oracle_finished_same in H7; eauto; subst.
+    edestruct H; eauto.
+    eapply_fresh H2 in H10; cleanup.
+    eapply_fresh Hx in H7; logic_clean.
+    clear H3 H6.
+    exists (o1++x0).
+    unfold minimal_oracle; intros.
+    eexists; intros.
+    rewrite <- app_assoc; eauto.
+    intuition eauto.
+    econstructor; eauto.
+    inversion H3; cleanup.
+    {
+      eapply exec_finished_deterministic_prefix in H7; eauto; cleanup.
+      eapply H2 in H18; logic_clean; eauto.
+    }
+    {
+      exfalso; 
+      eapply finished_not_crashed_oracle_prefix; [eauto | | eauto].
+      rewrite <- app_assoc; eauto.
+    }
+    {
+      rewrite app_length in *.
+    destruct (PeanoNat.Nat.eq_dec n (length o1)).
+
+    rewrite firstn_app_l in H9; eauto.
+    rewrite firstn_oob in H9; eauto.
+    inversion H9; subst; sigT_eq.
+    eapply exec_finished_deterministic_prefix in H7; eauto.
+    logic_clean.
+    
+    assert (length o0 = length o0 + length o2). {
+      rewrite H7 at 1.
+      rewrite app_length; eauto.
+    }
+    assert (length o2 = 0). { lia. }
+    apply length_zero_iff_nil in H14; subst;
+    eapply exec_empty_oracle; eauto.
+    rewrite <- app_assoc; eauto.
+
+    eapply finished_not_crashed_oracle_prefix. 
+    apply H7.
+    2: eauto.
+    eauto.
+    all: try lia.
+    
+    apply PeanoNat.Nat.lt_gt_cases in n0.
+    destruct n0.
+    {
+      rewrite firstn_app_l in H9; eauto.
+      inversion H9; subst; sigT_eq.
+      destruct o2.
+      eapply exec_empty_oracle; eauto.
+      assert (exists m, o0 = firstn m o1 /\ m < length o1). {
+      rewrite <- firstn_skipn with (n:= length o0) in H12.
+      eapply app_split_length_eq_l in H12. 
+      logic_clean; subst.
+      rewrite firstn_firstn in H12.
+      eexists; eauto.
+      split; eauto.
+      eapply PeanoNat.Nat.min_lt_iff; eauto.
+      rewrite firstn_skipn in H12.
+      rewrite <- H12.
+      rewrite firstn_app2; eauto.
+    }
+    logic_clean; subst.
+    eapply H8; eauto.
+    eapply finished_not_crashed_oracle_prefix. 
+    apply H7.
+    2: eauto.
+    rewrite app_nil_r; eauto.
+    erewrite firstn_skipn; eauto.
+    repeat rewrite <- app_assoc; eauto.
+    lia.
+    }
+    {
+      rewrite firstn_app_le in H9.
+    inversion H9; subst; sigT_eq.
+    eapply exec_finished_deterministic_prefix in H7; eauto.
+    logic_clean; subst; clear_lists; subst.
+    eapply H5; eauto.
+    lia.
+    eapply finished_not_crashed_oracle_prefix in H7; eauto.
+    repeat rewrite <- app_assoc; eauto.
+    lia.
+    }
+  }
+  {
+    edestruct IHp; eauto.
+    apply H1 in H6; eauto; cleanup.
+    exists x; intuition eauto.
+    unfold minimal_oracle; intros.
+    eapply exec_deterministic_wrt_oracle in H0; eauto; cleanup.
+    eexists; intuition eauto.
+    eapply ExecBindCrash; eauto.
+    inversion H5; cleanup.
+    {
+    eapply finished_not_crashed_oracle_prefix. 
+    apply H12.
+    2: eauto.
+    setoid_rewrite app_nil_r at 2; eauto.
+    instantiate (1:= o2 ++ skipn n x).
+    erewrite <- firstn_skipn with (l:= x) at 2.
+    rewrite <- H6.
+    repeat rewrite <- app_assoc; eauto.
+    }
+    {
+      eauto.
+    }
+    }
+  }
+  
+  Unshelve.
+  all:  eauto.
+Qed.
+
+Lemma minimal_oracle_unique :
+forall O (L: Language O) T (p: prog L T) u o om1 om2 s r,
+exec L u o s p r ->
+minimal_oracle p u s o om1 ->
+minimal_oracle p u s o om2 ->
+om1 = om2.
+Proof.
+  intros.
+  eapply_fresh H0 in H; cleanup.
+  eapply_fresh H1 in H; cleanup.
+  destruct (PeanoNat.Nat.eq_dec (length om1) (length om2)).
+  eapply app_split_length_eq_l in H2; eauto; cleanup; eauto.
+
+  apply PeanoNat.Nat.lt_gt_cases in n.
+  destruct n.
+  {
+    assert (exists m, om1 = firstn m om2 /\ m < length om2). {
+    rewrite <- firstn_skipn with (n:= length om1) in H2.
+    eapply app_split_length_eq_l in H2. 
+    logic_clean; subst.
+    rewrite firstn_app_l in H2.
+    eexists; eauto.
+    lia.
+    rewrite firstn_length_l; eauto.
+    rewrite app_length; lia.
+  }
+  logic_clean; subst.
+  exfalso; eapply H6; eauto.
+  }
+  {
+    assert (exists m, om2 = firstn m om1 /\ m < length om1). {
+    rewrite <- firstn_skipn with (n:= length om2) (l:= om1) in H2.
+    rewrite <- app_assoc in H2.
+    eapply app_split_length_eq_l in H2. 
+    logic_clean; subst.
+    eexists; eauto.
+    rewrite firstn_length_l; eauto; lia.
+  }
+  logic_clean; subst.
+  exfalso; eapply H4; eauto.
+  }
+Qed.
+
+Lemma exec_crashed_minimal_oracle:
+  forall O (L: Language O) T (p: prog L T) u o s s',
+      exec L u o s p (Crashed s') ->
+      exists o1 o2,
+      o = o1 ++ o2 /\
+      exec L u o1 s p (Crashed s') /\
+      (forall n r, 
+      n < length o1 ->
+      ~ exec L u (firstn n o1) s p r).
+Proof.
+  intros; eapply_fresh minimal_oracle_exists in H; cleanup.
+  eapply H0 in H; cleanup.
+  do 2 eexists; intuition eauto.
+Qed.
