src/Framework/Simulation/HorizontalCompositionRefinement.v
@@ -1,0 +1,294 @@
+Require Import List Primitives Layer.
+Require Import Simulation.Definitions RefinementLift. 
+Import ListNotations.
+
+Set Implicit Arguments.
+
+Section HC_Refinement.
+
+Variable O O1 O2: Core.
+Variable L1 : Language O1.
+Variable L2 : Language O2.
+Variable HCL1 : Language (HorizontalComposition O O1).
+Variable HCL2 : Language (HorizontalComposition O O2).
+Variable RC: CoreRefinement L1 O2.
+
+Definition compile T (o: (HorizontalComposition O O2).(operation) T) : HCL1.(prog) T := 
+    match o with
+    | P1 p1 => Op (HorizontalComposition O O1) (P1 p1)
+    | P2 p2 => lift_L2 _ (RC.(compile_core) p2)
+    end.
+
+Definition HC_refines := fun (si: HCL1.(state)) (sa: HCL2.(state)) => 
+fst si = fst sa /\ RC.(refines_core) (snd si) (snd sa).
+
+Lemma HC_exec_compiled_preserves_refinement_finished_core :
+forall T (p2: (HorizontalComposition O O2).(operation) T) o1 s1 s1' r u,
+  (exists s2, HC_refines s1 s2) ->
+  HCL1.(exec) u o1 s1 (compile p2) (Finished s1' r) ->
+  (exists s2', HC_refines s1' s2').
+  Proof.
+    destruct p2; simpl; intros.
+    {
+        unfold HC_refines in *; cleanup;
+        repeat invert_exec.
+        simpl; exists (s0, snd x); split; eauto.
+    }
+    {
+        unfold HC_refines in *; cleanup; 
+        repeat invert_exec; eauto.
+        eapply RC.(exec_compiled_preserves_refinement_finished_core) in H3; eauto.
+        cleanup.
+        simpl; exists (fst s1, x1); split; eauto.
+    }
+Qed.
+
+Fixpoint HC_oracle_transformation (o1: oracle HCL1) (o2: oracle L1) :=
+match o1 with
+| [] => o2 = []
+| t1::o1' => 
+    match t1 with
+    | OpToken _ t =>
+        exists t' o2', 
+        t = Token2 _ _ t' /\
+        o2 = (OpToken _ t') :: o2' /\
+        HC_oracle_transformation o1' o2'
+    | Cont _ =>
+        exists o2', 
+        o2 = (Cont _):: o2' /\
+        HC_oracle_transformation o1' o2'
+    | Crash _ =>
+        exists o2', 
+        o2 = (Crash _):: o2' /\
+        HC_oracle_transformation o1' o2'
+    end
+end.
+
+
+(* Problem Here is A single token in abstract turns into an oracle for implementation, it is like flattened *)
+Definition HC_token_refines T u (d1: HCL1.(state)) 
+(p: (HorizontalComposition O O2).(operation) T) 
+(get_reboot_state: HCL1.(state) -> HCL1.(state)) (o1: oracle HCL1) t2 : Prop :=
+match p with
+| P1 p1 => exists t , t2 = Token1 _ _ t /\ o1 = [OpToken (HorizontalComposition O O1) (Token1 O O1 t)] 
+| P2 p2 =>
+    exists t o grs1, t2 = Token2 _ _ t /\ 
+    (* @minimal_oracle _ HCL1 _ (lift_L2 O (compile_core RC p2)) u d1 o1 om1 /\ *)
+    HC_oracle_transformation o1 o /\
+    RC.(token_refines) u (snd d1) p2 grs1 o t
+end.
+    
+
+Definition HC_Core_Refinement : CoreRefinement HCL1 (HorizontalComposition O O2) :=
+Build_CoreRefinement compile HC_refines
+HC_token_refines
+HC_exec_compiled_preserves_refinement_finished_core.
+
+Definition HC_Refinement := LiftRefinement HCL2 HC_Core_Refinement.
+
+
+Lemma HC_oracle_transformation_id:
+forall o1 o2,
+HC_oracle_transformation
+(map
+    (fun o : Language.token' O1 =>
+    match o with
+    | OpToken _ o1 =>
+        OpToken (HorizontalComposition O O1)
+          (Token2 O O1 o1)
+    | Language.Crash _ =>
+        Language.Crash (HorizontalComposition O O1)
+    | Language.Cont _ =>
+        Language.Cont (HorizontalComposition O O1)
+    end) o1) o2 ->
+    o1 = o2.
+  Proof.
+    induction o1; simpl; intros; eauto.
+    {
+      destruct a; simpl; cleanup; eauto.
+      inversion H; subst.
+      all: erewrite IHo1; eauto.
+    }
+  Qed.
+
+Lemma HC_oracle_transformation_id_crashed:
+forall o1 o2 o,
+HC_oracle_transformation
+(map
+    (fun o : Language.token' O1 =>
+    match o with
+    | OpToken _ o1 =>
+        OpToken (HorizontalComposition O O1)
+          (Token2 O O1 o1)
+    | Language.Crash _ =>
+        Language.Crash (HorizontalComposition O O1)
+    | Language.Cont _ =>
+        Language.Cont (HorizontalComposition O O1)
+    end) o1 ++ o) o2 ->
+    exists o2' rest,
+    o2 = o2'++rest /\
+    o1 = o2' /\ HC_oracle_transformation o rest.
+  Proof.
+    induction o1; simpl; intros; eauto.
+    do 2 eexists; simpl; intuition eauto.
+    simpl; eauto.
+    {
+      destruct a; simpl; cleanup; eauto.
+      inversion H; subst.
+
+      edestruct IHo1; eauto; cleanup; eauto.
+      do 2 eexists; intuition eauto.
+      simpl; eauto.
+
+      edestruct IHo1; eauto; cleanup; eauto.
+      do 2 eexists; intuition eauto.
+      simpl; eauto.
+
+      edestruct IHo1; eauto; cleanup; eauto.
+      do 2 eexists; intuition eauto.
+      simpl; eauto.
+    }
+  Qed.
+
+  Lemma HC_oracle_transformation_app:
+forall x0 x1 x2,
+HC_oracle_transformation  x0 (x1 ++ x2) ->
+exists x x',
+x0 = x ++ x' /\
+x = map
+(fun o : Language.token' O1 =>
+    match o with
+    | OpToken _ o1 =>
+        OpToken (HorizontalComposition O O1)
+          (Token2 O O1 o1)
+    | Language.Crash _ =>
+        Language.Crash (HorizontalComposition O O1)
+    | Language.Cont _ =>
+        Language.Cont (HorizontalComposition O O1)
+    end) x1 /\ 
+  HC_oracle_transformation x' x2.
+  Proof.
+    induction x0; simpl; intros; eauto.
+    {
+      exists [], [].
+      apply app_eq_nil in H; cleanup.
+      simpl; intuition eauto.
+    }
+    {
+    cleanup; eauto.
+    {
+      destruct x1.
+      {
+        exists []; simpl in *; eexists; intuition.
+        cleanup; simpl.
+        do 2 eexists; intuition eauto.
+      }
+      {
+        simpl in *; cleanup.
+        eapply IHx0 in H1; eauto; cleanup.
+        do 2 eexists; intuition eauto.
+        simpl; eauto.
+      }
+    }
+    {
+      destruct x1.
+      {
+        exists []; simpl in *; eexists; intuition.
+        cleanup; simpl.
+        do 2 eexists; intuition eauto.
+      }
+      {
+        simpl in *; cleanup.
+        eapply IHx0 in H0; eauto; cleanup.
+        do 2 eexists; intuition eauto.
+        simpl; eauto.
+      }
+    }
+    {
+      destruct x1.
+      {
+        exists []; simpl in *; eexists; intuition.
+        cleanup; simpl.
+        do 2 eexists; intuition eauto.
+      }
+      {
+        simpl in *; cleanup.
+        eapply IHx0 in H0; eauto; cleanup.
+        do 2 eexists; intuition eauto.
+        simpl; eauto.
+      }
+    }
+    }
+  Qed.
+
+  Lemma HC_oracle_transformation_same:
+    forall 
+      (o1 : list (Language.token' O1)),
+    HC_oracle_transformation 
+      (map
+          (fun o : Language.token' O1 =>
+          match o with
+          | OpToken _ o3 =>
+              OpToken (HorizontalComposition O O1) (Token2 O O1 o3)
+          | Language.Crash _ => Language.Crash (HorizontalComposition O O1)
+          | Language.Cont _ => Language.Cont (HorizontalComposition O O1)
+          end) o1) o1.
+    Proof.
+      induction o1; simpl; intros; eauto.
+      destruct a; simpl; intuition eauto.
+    Qed.
+
+
+Lemma HC_oracle_transformation_id_rev:
+forall T (p: L1.(prog) T) x0 u x3 s s' r,
+HC_oracle_transformation x0 x3 ->
+exec L1 u x3 s p (Finished s' r) ->
+x0 = map
+(fun o : Language.token' O1 =>
+    match o with
+    | OpToken _ o1 =>
+        OpToken (HorizontalComposition O O1)
+          (Token2 O O1 o1)
+    | Language.Crash _ =>
+        Language.Crash (HorizontalComposition O O1)
+    | Language.Cont _ =>
+        Language.Cont (HorizontalComposition O O1)
+    end) x3.
+  Proof.
+    induction p; simpl; intros.
+    {
+      unfold HC_oracle_transformation in *.
+      invert_exec.
+      simpl in *.
+      destruct x0; eauto.
+      congruence.
+      cleanup; simpl in *.
+      destruct x0; cleanup; try congruence.
+    }
+    {
+    unfold HC_oracle_transformation in *.
+    invert_exec.
+    simpl in *.
+    destruct x0; eauto.
+    congruence.
+    cleanup; simpl in *.
+    destruct x0; cleanup; congruence.
+    }
+    {
+    invert_exec.
+    simpl in *.
+    eapply HC_oracle_transformation_app in H0; cleanup.
+    edestruct IHp.
+    2: eauto.
+    apply HC_oracle_transformation_same.
+    erewrite H with (x0 := x5); eauto.
+    rewrite map_app; eauto.
+    }
+  Qed.
+
+End HC_Refinement.
+
+Arguments HC_Refinement {_ _ _ _}.
+
+
+
