src/Framework/Simulation/RefinementLift.v
@@ -1,4 +1,4 @@
-Require Import Primitives Layer Simulation.Definitions.
+Require Import Primitives Layer Simulation.Definitions Lia.
 
 Section RefinementLift.
   Variable C_imp C_abs: Core.
@@ -59,7 +59,279 @@ Section RefinementLift.
       oracle_refines
       exec_compiled_preserves_refinement_finished.
 
+(*
+Theorem SimulationForProgram_compositional_lifted:
+      forall u l_grsi_1  l_grsa_1  T (p1_abs: L_abs.(prog) T) 
+      T' (p2_abs: T -> L_abs.(prog) T') (rec_abs : L_abs.(prog) unit),
+      SimulationForProgram LiftRefinement u p1_abs rec_abs [] [] ->
+      SimulationForProgram LiftRefinement u p1_abs rec_abs l_grsi_1 l_grsa_1 ->
+      (forall t, SimulationForProgram LiftRefinement u (p2_abs t) rec_abs l_grsi_1 l_grsa_1) ->
+      SimulationForProgram LiftRefinement u (Bind p1_abs p2_abs) rec_abs l_grsi_1 l_grsa_1.
+Proof.
+  unfold SimulationForProgram, SimulationForProgramGeneral; intros.
+  simpl in *. repeat invert_exec; simpl in *.
+  {
+    cleanup; try intuition; try lia; simpl in *.
+    {
+      destruct l; simpl in *; try lia.
+      cleanup; unify_execs; cleanup.
+      invert_exec'' H13.
+      split_ors; cleanup; repeat unify_execs; cleanup.
+      eapply exec_deterministic_wrt_oracle_prefix in H4; eauto; cleanup.
+      eapply exec_finished_deterministic_prefix in H4; eauto; cleanup.
+      unify_execs; cleanup.
+
+      edestruct H0; eauto.
+      instantiate (1:= [x3]).
+      instantiate (1:= [x1]).
+      simpl; eauto.
+      split; eauto.
+      left; do 2 eexists; 
+      split; eauto.
+      econstructor; eauto.
+      simpl in *; cleanup.
+      destruct x7; simpl in *; cleanup.
+
+      edestruct H1; eauto.
+      instantiate (1:= [x4]).
+      instantiate (1:= [x2]).
+      simpl; eauto.
+      split; eauto.
+      left; do 2 eexists; 
+      split; eauto.
+      econstructor; eauto.
+      simpl in *; cleanup.
+      destruct x6; simpl in *; cleanup.
+
+      exists (RFinished s0 t0).
+      inversion H2; cleanup.
+      inversion H5; cleanup.
+      split; simpl; eauto.
+      eapply ExecFinished; eauto.
+      econstructor; eauto.
+  }
+  cleanup; intuition.
+}
+{
+  cleanup; try intuition; simpl in *;
+  cleanup; unify_execs; cleanup.
+  invert_exec'' H12.
+  {
+    split_ors; cleanup; repeat unify_execs; cleanup.
+    eapply exec_deterministic_wrt_oracle_prefix in H5; eauto; cleanup.
+    eapply exec_finished_deterministic_prefix in H5; eauto; cleanup.
+    unify_execs; cleanup.
+
+    edestruct H; eauto.
+    instantiate (1:= [x2]).
+    instantiate (1:= [x0]).
+    simpl; eauto.
+    split; eauto.
+    left; do 2 eexists; 
+    split; eauto.
+    econstructor; eauto.
+    simpl in *; cleanup.
+    destruct x6; simpl in *; cleanup.
+
+    edestruct H1; eauto.
+    instantiate (1:= x3 :: l).
+    instantiate (1:= x1 :: lo).
+    simpl; eauto.
+    split; eauto.
+    econstructor; eauto.
+    simpl in *; cleanup.
+    destruct x5; simpl in *; cleanup.
+
+    exists (Recovered s0); split; eauto.
+    inversion H4; cleanup.
+    inversion H7; cleanup.
+    econstructor; eauto.
+    econstructor; eauto.
+  }
+  {
+    split_ors; cleanup; repeat unify_execs; cleanup.
+    eapply_fresh exec_deterministic_wrt_oracle_prefix in H5; eauto; cleanup.
+
+    edestruct H0; eauto.
+    instantiate (1:= x2::l).
+    instantiate (1:= x0::lo).
+    simpl; eauto.
+    split; eauto.
+    econstructor; eauto.
+    simpl in *; cleanup.
+    destruct x; simpl in *; cleanup.
+
+    exists (Recovered s); split; eauto.
+    inversion H8; cleanup.
+    econstructor; eauto.
+    eapply ExecBindCrash; eauto.
+  }
+}
+Qed.
+*)
+Lemma abstract_oracles_exist_wrt_compositional:
+forall u l_grs T (p1: prog L_abs T) T' (p2: T -> prog L_abs T') rec, 
+abstract_oracles_exist_wrt LiftRefinement LiftRefinement.(refines) u p1 rec [] ->
+abstract_oracles_exist_wrt LiftRefinement LiftRefinement.(refines) u p1 rec l_grs ->
+(forall t, abstract_oracles_exist_wrt LiftRefinement LiftRefinement.(refines) u (p2 t) rec l_grs) ->
+abstract_oracles_exist_wrt LiftRefinement LiftRefinement.(refines) u (Bind p1 p2) rec l_grs.
+Proof.
+    unfold abstract_oracles_exist_wrt; 
+    simpl; intros;
+    repeat invert_exec.
+    {
+        invert_exec'' H12.
+        edestruct H; eauto.
+        econstructor; eauto.
+
+        eapply_fresh exec_compiled_preserves_refinement_finished in H9; eauto.
+
+        edestruct H1; eauto.
+        econstructor; eauto.
+
+        simpl in *; cleanup; try intuition; simpl in *; try congruence;
+        cleanup; repeat unify_execs; cleanup.
+        exists [o0++o].
+        simpl; split; eauto.
+        repeat left.
+        do 2 eexists; econstructor; eauto.
+        econstructor; eauto.
+        intuition eauto.
+        do 4 eexists; intuition eauto. 
+        right; do 3 eexists; intuition eauto.
+    }
+    {
+        invert_exec'' H11.
+        {
+            edestruct H; eauto.
+            econstructor; eauto.
+
+            eapply_fresh exec_compiled_preserves_refinement_finished in H9; eauto.
+
+            edestruct H1; eauto.
+            econstructor; eauto.
+
+            simpl in *; cleanup; try intuition; simpl in *; try congruence;
+            cleanup; repeat unify_execs; cleanup.
+            exists ((o0++o)::l).
+            simpl; split; eauto.
+            right.
+            eexists; econstructor; eauto.
+            econstructor; eauto.
+            intuition eauto.
+            do 4 eexists; intuition eauto. 
+            right; do 3 eexists; intuition eauto.
+        }
+        {
+            edestruct H0; eauto.
+            econstructor; eauto.
+
+            simpl in *; cleanup; try intuition; simpl in *; try congruence;
+            cleanup; repeat unify_execs; cleanup.
+            eexists (_::l).
+            simpl; split; eauto.
+            right.
+            eexists; econstructor; eauto.
+            eapply ExecBindCrash; eauto.
+            intuition eauto.
+            do 4 eexists; intuition eauto. 
+            rewrite app_nil_r; eauto.
+        }
+    }
+    Unshelve.
+    eauto.
+Qed.
+
+(*
+Lemma oracle_refines_same_from_related_compositional:
+forall u R l_grs T (p1 p2: prog L_abs T) T' (p3 p4: T -> prog L_abs T') rec, 
+oracle_refines_same_from_related LiftRefinement u p1 p2 rec [] R ->
+oracle_refines_same_from_related LiftRefinement u p1 p2 rec l_grs R ->
+(forall t t', oracle_refines_same_from_related LiftRefinement u (p3 t) (p4 t') rec l_grs R) ->
+oracle_refines_same_from_related LiftRefinement u (Bind p1 p3) (Bind p2 p4) rec l_grs R.
+Proof.
+    unfold oracle_refines_same_from_related; 
+    simpl; intros.
+    destruct l_o_imp; simpl in *; intuition.
+
+    cleanup; try intuition simpl in *; try congruence; try lia.
+    {  
+      repeat split_ors; cleanup.
+      invert_exec'' H0.
+      invert_exec'' H5.
+      repeat split_ors; cleanup; repeat unify_execs; cleanup;
+      eapply_fresh exec_deterministic_wrt_oracle_prefix in H5; eauto; cleanup;
+      eapply_fresh exec_deterministic_wrt_oracle_prefix in H7; eauto; cleanup.
+      rewrite H4; eauto.  
+      eapply_fresh exec_finished_deterministic_prefix in H5; eauto; cleanup;
+      eapply_fresh exec_finished_deterministic_prefix in H7; eauto; cleanup.
+      rewrite <- H4 in H6; clear H4; cleanup; repeat unify_execs; cleanup.
+
+
+      }
+      invert_exec'' H12.
+        edestruct H; eauto.
+        econstructor; eauto.
+
+        eapply_fresh exec_compiled_preserves_refinement_finished in H9; eauto.
+
+        edestruct H1; eauto.
+        econstructor; eauto.
+
+        simpl in *; cleanup; try intuition; simpl in *; try congruence;
+        cleanup; repeat unify_execs; cleanup.
+        exists [o0++o].
+        simpl; split; eauto.
+        repeat left.
+        do 2 eexists; econstructor; eauto.
+        econstructor; eauto.
+        intuition eauto.
+        do 4 eexists; intuition eauto. 
+        right; do 3 eexists; intuition eauto.
+    }
+    {
+        invert_exec'' H11.
+        {
+            edestruct H; eauto.
+            econstructor; eauto.
+
+            eapply_fresh exec_compiled_preserves_refinement_finished in H9; eauto.
+
+            edestruct H1; eauto.
+            econstructor; eauto.
+
+            simpl in *; cleanup; try intuition; simpl in *; try congruence;
+            cleanup; repeat unify_execs; cleanup.
+            exists ((o0++o)::l).
+            simpl; split; eauto.
+            right.
+            eexists; econstructor; eauto.
+            econstructor; eauto.
+            intuition eauto.
+            do 4 eexists; intuition eauto. 
+            right; do 3 eexists; intuition eauto.
+        }
+        {
+            edestruct H0; eauto.
+            econstructor; eauto.
+
+            simpl in *; cleanup; try intuition; simpl in *; try congruence;
+            cleanup; repeat unify_execs; cleanup.
+            exists (o::l).
+            simpl; split; eauto.
+            right.
+            eexists; econstructor; eauto.
+            eapply ExecBindCrash; eauto.
+            intuition eauto.
+            do 4 eexists; intuition eauto. 
+            rewrite app_nil_r; eauto.
+        }
+    }
+Qed.
+*)
+
 End RefinementLift.
 
 Arguments LiftRefinement {_ _ _}.
-
+(* Arguments SimulationForProgram_compositional_lifted {_ _ _ _}. *)
+Arguments abstract_oracles_exist_wrt_compositional {_ _ _ _}.
