src/Noninterference/FileDisk/SSE/InodeSSE.v
@@ -625,6 +625,36 @@ Proof.
   lia.
 Qed.
 
+
+  Lemma count_trues_upd:
+  forall l a,
+  seln l a false = false ->
+  a < length l ->
+  count_trues (updn l a true) = S (count_trues l).
+  Proof.
+    induction l; simpl; intros; try lia.
+    destruct a0; simpl in *; subst; eauto.
+    destruct a; eauto;
+    erewrite IHl; eauto; lia.
+  Qed.
+
+  Lemma count_trues_upd_list:
+  forall l_a l,
+  (forall a, In a l_a -> seln l a false = false) ->
+  Forall (fun a => a < length l) l_a ->
+  NoDup l_a -> 
+  count_trues (repeated_apply (fun l a => updn l a true) l l_a) = length l_a + count_trues l.
+  Proof.
+    induction l_a; simpl; intros; try lia.
+    inversion H0; clear H0; subst.
+    inversion H1; clear H1; subst.
+    erewrite count_trues_upd.
+    rewrite IHl_a; eauto.
+    erewrite seln_repeated_apply_updn; eauto.
+    rewrite repeated_apply_length; intros; eauto.
+    apply updn_length.
+  Qed.
+
 Set Nested Proofs Allowed.
 Lemma count_trues_ge_all_some:
 forall l bm s,
@@ -632,7 +662,188 @@ DiskAllocator.block_allocator_rep bm s ->
 Forall (fun a => bm a <> None) l ->
 NoDup l ->
 count_trues (firstn DiskAllocatorParams.num_of_blocks (value_to_bits (s DiskAllocatorParams.bitmap_addr)) ) >= length l.
-Proof. Admitted.
+Proof. 
+  induction l; simpl; intros.
+  lia.
+  inversion H0; inversion H1; 
+  clear H0 H1; cleanup.  eapply_fresh DiskAllocator.block_allocator_rep_delete with (a:= a) in H.
+  assert (A: Forall (fun ax : addr => (Mem.delete bm a) ax <> None) l). {
+    eapply Forall_forall; intros.
+    destruct (PeanoNat.Nat.eq_dec a x); subst.
+    tauto.
+    rewrite delete_ne; eauto.
+    eapply Forall_forall in H5; eauto.
+  }
+  specialize (IHl _ _ Hx A H9).
+  clear Hx.
+  unfold DiskAllocator.block_allocator_rep in *; cleanup.
+  eapply DiskAllocator.valid_bits_extract with (n:= a) in H0; eauto.
+  cleanup; split_ors; cleanup; try congruence.
+
+  replace (firstn DiskAllocatorParams.num_of_blocks
+  (value_to_bits (s DiskAllocatorParams.bitmap_addr))) with
+  (updn (firstn DiskAllocatorParams.num_of_blocks
+  (value_to_bits
+     (upd s DiskAllocatorParams.bitmap_addr
+        (bits_to_value
+           (updn (value_to_bits (s DiskAllocatorParams.bitmap_addr))
+              a false)) DiskAllocatorParams.bitmap_addr))) a true).
+
+  erewrite count_trues_upd.
+  lia.
+  rewrite seln_firstn.
+  rewrite upd_eq.
+  rewrite bits_to_value_to_bits_exact.
+  rewrite seln_updn_eq; eauto.
+  rewrite value_to_bits_length.
+  pose proof DiskAllocatorParams.num_of_blocks_in_bounds.
+  destruct (Compare_dec.lt_dec a DiskAllocatorParams.num_of_blocks).
+  unfold DiskAllocatorParams.num_of_blocks in *; lia.
+  rewrite H2 in H3; try congruence; lia.
+  rewrite updn_length, value_to_bits_length; eauto.
+  eauto.
+  destruct (Compare_dec.lt_dec a DiskAllocatorParams.num_of_blocks).
+  unfold DiskAllocatorParams.num_of_blocks in *; lia.
+  rewrite H2 in H3; try congruence; lia.
+  pose proof DiskAllocatorParams.num_of_blocks_in_bounds.
+  rewrite firstn_length_l.
+  destruct (Compare_dec.lt_dec a DiskAllocatorParams.num_of_blocks).
+  unfold DiskAllocatorParams.num_of_blocks in *; lia.
+  rewrite H2 in H3; try congruence; lia.
+  rewrite value_to_bits_length; unfold DiskAllocatorParams.num_of_blocks; eauto.
+  destruct (Compare_dec.lt_dec a DiskAllocatorParams.num_of_blocks); 
+  [|rewrite H2 in H3; try congruence; lia].
+  rewrite <- updn_firstn_comm.
+  rewrite upd_eq.
+  rewrite bits_to_value_to_bits_exact.
+  
+  rewrite updn_twice.
+  erewrite seln_eq_updn_eq; eauto.
+  rewrite updn_length, value_to_bits_length; eauto.
+  eauto.
+  destruct (Compare_dec.lt_dec a DiskAllocatorParams.num_of_blocks).
+  unfold DiskAllocatorParams.num_of_blocks in *; lia.
+  rewrite H2 in H4; try congruence; lia.
+  pose proof DiskAllocatorParams.num_of_blocks_in_bounds.
+  rewrite value_to_bits_length;
+  rewrite H1; unfold DiskAllocatorParams.num_of_blocks; eauto.
+Qed.
+
+
+Lemma file_map_rep_delete_file:
+      forall fm im bm s f i inum,
+      file_map_rep fm im bm ->
+      Inode.inode_rep im s ->
+      DiskAllocator.block_allocator_rep bm s ->
+      fm inum = Some f ->
+      im inum = Some i ->
+      let bm' := (repeated_apply (Mem.delete (AEQ:=addr_dec)) bm (Inode.block_numbers i)) in
+      let s' := (upd (upd s DiskAllocatorParams.bitmap_addr
+                     (bits_to_value
+                        (repeated_apply (fun (l : list bool) (a : nat) => updn l a false)
+                                        (value_to_bits (s DiskAllocatorParams.bitmap_addr)) (Inode.block_numbers i)))) Inode.InodeAllocatorParams.bitmap_addr
+                (bits_to_value
+                        (updn (value_to_bits (s Inode.InodeAllocatorParams.bitmap_addr)) inum false)))  in
+ 
+ file_map_rep (Mem.delete fm inum) (Mem.delete im inum) bm' /\
+ Inode.inode_rep (Mem.delete im inum) s' /\
+ DiskAllocator.block_allocator_rep bm' s'.
+    Proof.
+      unfold file_map_rep, file_rep, 
+    Inode.inode_rep, Inode.inode_map_rep,
+    Inode.inode_map_valid, Inode.inode_valid in *;
+      intros; cleanup.
+      eapply_fresh H7 in H2; eauto; cleanup.
+      eapply_fresh H5 in H3; cleanup.
+      split.
+      2: split.
+      {(** file_map_rep **)
+       intuition.
+        {
+            unfold addrs_match_exactly in *; intros.
+            destruct (addr_dec inum a); subst.
+            repeat rewrite Mem.delete_eq; eauto.
+            split; intros; congruence.
+            repeat rewrite Mem.delete_ne; eauto.
+          }
+          {
+            destruct (addr_dec inum inum0); subst;
+            [rewrite Mem.delete_eq in H13;
+             rewrite Mem.delete_eq in H14; eauto |
+             rewrite Mem.delete_ne in H13;
+             rewrite Mem.delete_ne in H14; eauto];
+            try congruence.
+            eapply_fresh H7 in H13; eauto.
+            unfold file_rep in *; cleanup; eauto.
+          }
+          {
+            destruct (addr_dec inum inum0); subst;
+            [rewrite Mem.delete_eq in H13;
+             rewrite Mem.delete_eq in H14; eauto |
+             rewrite Mem.delete_ne in H13;
+             rewrite Mem.delete_ne in H14; eauto];
+            try congruence.
+            eapply_fresh H7 in H13; eauto.
+            unfold file_rep in *; cleanup; eauto.
+          }
+          {
+            destruct (addr_dec inum inum0); subst;
+            [rewrite Mem.delete_eq in H13;
+             rewrite Mem.delete_eq in H14; eauto |
+             rewrite Mem.delete_ne in H13;
+             rewrite Mem.delete_ne in H14; eauto];
+            try congruence.
+            {
+              eapply_fresh H6 in H13; eauto.
+              eapply_fresh H7 in H13; eauto.
+              cleanup.
+              eapply_fresh H18 in H15; eauto;
+              cleanup.
+              eexists; intuition eauto.
+              eapply nth_error_In in H15.
+              eapply not_In_NoDup_app in H15; eauto.
+              rewrite repeated_apply_delete_not_in; eauto.
+            }
+          }
+        }
+      {(** inode_rep **)
+        eexists; intuition eauto.
+        rewrite upd_comm.
+        eapply Inode.InodeAllocator.block_allocator_rep_upd_noop; eauto.
+        eapply Inode.InodeAllocator.block_allocator_rep_delete; eauto.
+        unfold DiskAllocatorParams.bitmap_addr,
+        Inode.InodeAllocatorParams.bitmap_addr.
+        pose proof FSParameters.inodes_before_data; lia.
+        destruct (addr_dec inum i0); subst.
+        repeat rewrite Mem.delete_eq; simpl; eauto.
+        repeat rewrite Mem.delete_ne; simpl; eauto.
+        
+        destruct (addr_dec inum i0); subst.
+        rewrite Mem.delete_eq in H13; simpl; congruence.
+        rewrite Mem.delete_ne in H13; simpl; eauto.
+        eapply H5 in H13; cleanup; eauto.
+
+        destruct (addr_dec inum i0); subst.
+        rewrite Mem.delete_eq in H13; simpl; congruence.
+        rewrite Mem.delete_ne in H13; simpl; eauto.
+        eapply H5 in H13; cleanup; eauto.
+
+        destruct (addr_dec inum i0); subst.
+        rewrite Mem.delete_eq in H14; simpl; congruence.
+        rewrite Mem.delete_ne in H14; simpl; eauto.
+        destruct (addr_dec inum j); subst.
+        rewrite Mem.delete_eq in H15; simpl; congruence.
+        rewrite Mem.delete_ne in H15; simpl; eauto.
+      }
+      {
+       eapply DiskAllocator.block_allocator_rep_upd_noop; eauto.
+       eapply DiskAllocator.block_allocator_rep_delete_list; eauto.
+        unfold DiskAllocatorParams.bitmap_addr,
+        Inode.InodeAllocatorParams.bitmap_addr.
+        pose proof FSParameters.inodes_before_data; lia.
+      }
+
+    Qed.
 
 
 Lemma block_counts_up_to_le:
@@ -644,11 +855,12 @@ count_trues (firstn DiskAllocatorParams.num_of_blocks
 (value_to_bits (s DiskAllocatorParams.bitmap_addr))) >=
 get_all_file_sizes_up_to fm n.
 Proof.
-  unfold file_map_rep, file_rep, 
-  Inode.inode_rep, Inode.inode_map_rep,
-  Inode.inode_map_valid, Inode.inode_valid;
   induction n; simpl; intros; cleanup.
   {
+    unfold file_map_rep, file_rep, 
+    Inode.inode_rep, Inode.inode_map_rep,
+    Inode.inode_map_valid, Inode.inode_valid in *;
+    cleanup.
     destruct_fresh (fm 0); try lia.
     destruct_fresh (im 0).
     {
@@ -665,12 +877,39 @@ Proof.
     edestruct H; exfalso.
     eapply H6; eauto; congruence.
   }
-  admit.
+  {
+    destruct_fresh (fm (S n)); try lia.
+    destruct_fresh (im (S n)).
+    {
+      eapply file_map_rep_delete_file in H; eauto.
+      cleanup.
+      eapply IHn in H; eauto.
+      rewrite upd_ne in H.
+      rewrite upd_eq in H; eauto.
+      rewrite bits_to_value_to_bits_exact in H.
+      (*
+      replace (firstn DiskAllocatorParams.num_of_blocks
+                      (value_to_bits (s DiskAllocatorParams.bitmap_addr))) with
+      (_).
+    
+      eapply count_trues_ge_all_some; eauto.
+      eapply Forall_forall; intros.
+      eapply in_seln_exists in H11; cleanup.
+      rewrite nth_seln_eq in H12.
+      eapply nth_error_nth' in H11.
+      apply H8 in H11; cleanup; try congruence.
+      rewrite H12 in H13; congruence.
+    }
+    edestruct H; exfalso.
+    eapply H6; eauto; congruence.
+    
+  }
   Unshelve.
   all: eauto.
+*)
 Admitted.
 
-Lemma block_counts_eq:
+Lemma block_counts_ge:
 forall n fm im bm s,
 file_map_rep fm im bm ->
 Inode.inode_rep im s ->
@@ -679,57 +918,7 @@ n >= FSParameters.inode_count ->
 count_trues (firstn DiskAllocatorParams.num_of_blocks
 (value_to_bits (s DiskAllocatorParams.bitmap_addr))) <=
 get_all_file_sizes_up_to fm n.
-Proof. (*
-  unfold file_map_rep, file_rep, 
-  Inode.inode_rep, Inode.inode_map_rep,
-  Inode.inode_map_valid, Inode.inode_valid;
-  induction n; intros; cleanup.
-  { pose proof FSParameters.inode_count_nonzero.
-  lia. }
-  {
-    inversion H2.
-    {
-      destruct_fresh (fm (S n)); simpl; eauto.
-      {
-        unfold Inode.InodeAllocator.block_allocator_rep in *; 
-        cleanup.
-        destruct_fresh (im (S n)).
-        rewrite H3, H10 in D0; eauto; simpl in *. 
-        congruence. 
-        unfold Inode.InodeAllocatorParams.num_of_blocks;
-        lia.
-        edestruct H; exfalso.
-        eapply H0; eauto; congruence.
-      }
-      {
-        rewrite H8; simpl; rewrite D; simpl.
-        erewrite get_all_file_sizes_equal_after_disk with (a:= 1).
-        replace (n + 1) with (S n) by lia.
-        eapply IHn; eauto.
-      }
-  }
-
-    destruct_fresh (fm 0); try lia.
-    destruct_fresh (im 0).
-    {
-      eapply_fresh H5 in D; eauto; cleanup.
-      eapply_fresh H3 in D0; cleanup.
-      eapply count_trues_ge_all_some; eauto.
-      eapply Forall_forall; intros.
-      eapply in_seln_exists in H11; cleanup.
-      rewrite nth_seln_eq in H12.
-      eapply nth_error_nth' in H11.
-      apply H8 in H11; cleanup; try congruence.
-      rewrite H12 in H13; congruence.
-    }
-    edestruct H; exfalso.
-    eapply H6; eauto; congruence.
-  }
-  admit.
-  Unshelve.
-  all: eauto.
-  *)
-Admitted.
+Proof. Admitted.
 
 Lemma block_counts_match:
 forall fm im bm s,
