src/Noninterference/TransactionalDisk/AbstractOraclesExist/ATCAOE.v
@@ -1,0 +1,624 @@
+Require Import Lia Framework ATCLayer File FileDiskNoninterference.
+
+Set Nested Proofs Allowed.
+
+(*
+Lemma HC_oracle_refines_2 :
+forall O O1 O2
+(L1: Language O1) (L2: Language O2)
+(HCL1: Language (HorizontalComposition O O1))
+(HCL2: Language (HorizontalComposition O O2))
+(RC: CoreRefinement L1 O2)
+u T p  s s0 x0 o,
+let R := LiftRefinement L2 RC in
+let HCR := HC_Refinement HCL1 HCL2 RC in
+(forall u s T (op:O2.(operation) T) o t, 
+token_refines RC u s op (fun s1 : state L1 => s1) o t ->
+minimal_oracle (compile_core RC op) u s o) ->
+oracle_refines O1 O2 L1 L2 RC T u s0 p (fun s1 : state L1 => s1) x0 o ->
+(forall T (p: L2.(prog) T), HCR.(Simulation.Definitions.compile) (lift_L2 _ p) = 
+lift_L2 _ (R.(Simulation.Definitions.compile) p)) ->
+oracle_refines (HorizontalComposition O O1) (HorizontalComposition O O2) HCL1
+HCL2 (HC_Core_Refinement HCL1 HCL2 RC) T u (s, s0) 
+(lift_L2 O p) (fun s1 : HorizontalComposition.state' O O1 => s1)
+(map
+(fun o0 : Language.token' O1 =>
+match o0 with
+| OpToken _ o1 => OpToken (HorizontalComposition O O1) (Token2 O O1 o1)
+| Language.Crash _ => Language.Crash (HorizontalComposition O O1)
+| Language.Cont _ => Language.Cont (HorizontalComposition O O1)
+end) x0)
+(map
+(fun o0 : Language.token' O2 =>
+match o0 with
+| OpToken _ o1 => OpToken (HorizontalComposition O O2) (Token2 O O2 o1)
+| Language.Crash _ => Language.Crash (HorizontalComposition O O2)
+| Language.Cont _ => Language.Cont (HorizontalComposition O O2)
+end) o).
+Proof.
+induction p; simpl; intros; cleanup.
+{
+  eexists; simpl; split; eauto.
+  do 5 eexists; intuition eauto.
+  setoid_rewrite app_nil_r; eauto.
+  apply HC_oracle_transformation_same; eauto.
+}
+{
+  split_ors; cleanup; invert_exec.
+  simpl; left; eexists; intuition eauto.
+  econstructor; eauto.
+  simpl; right; do 2 eexists; intuition eauto.
+  econstructor; eauto.
+}
+{
+  split_ors; cleanup.
+  {
+    repeat rewrite map_app; do 4 eexists; intuition eauto.
+    left; eexists; intuition eauto.
+    rewrite H2.
+    eapply lift2_exec_step_crashed; eauto.
+  }
+  {
+  repeat rewrite map_app; do 4 eexists; intuition eauto.
+  destruct x5;
+  right; do 3 eexists; intuition eauto.
+  rewrite H2; eapply lift2_exec_step; eauto.
+  rewrite H2; eapply lift2_exec_step; eauto.
+  rewrite H2; eapply lift2_exec_step; eauto.
+  rewrite H2; eapply lift2_exec_step_crashed; eauto.
+  }
+}
+Qed.
+*)
+(*
+Lemma HC_abstract_oracles_exist_wrt_2_recover:
+forall O O1 O2
+(L1: Language O1) (L2: Language O2)
+(HCL1: Language (HorizontalComposition O O1))
+(HCL2: Language (HorizontalComposition O O2))
+(RC: CoreRefinement L1 O2)
+(l_grs1: list (L1.(state) -> L1.(state))) 
+(l_grs2: list (HCL1.(state) -> HCL1.(state)))
+u (rec: HCL2.(prog) unit) 
+(rec2: L2.(prog) unit)
+refines_reboot,
+
+let R := LiftRefinement L2 RC in
+let HCR := HC_Refinement HCL1 HCL2 RC in
+
+abstract_oracles_exist_wrt R refines_reboot u rec2 rec2 l_grs1 ->
+Forall2 (fun f1 f2 => forall (s: (O.(Core.state) * L1.(state))), f1 (snd s) = snd (f2 s)) l_grs1 l_grs2 ->
+(HCR.(Simulation.Definitions.compile) (lift_L2 _ rec2) = lift_L2 _ (R.(Simulation.Definitions.compile) rec2)) ->
+
+(forall lo s ret grs1 grs2 l_grs1' l_grs2', 
+recovery_exec' u lo s l_grs2'
+(HCR.(Simulation.Definitions.compile) rec)
+(HCR.(Simulation.Definitions.compile) rec) ret ->
+l_grs1 = grs1::l_grs1' ->
+l_grs2 = grs2::l_grs2' ->
+exists lo' ret',
+   recovery_exec' u lo' (snd s) l_grs1' 
+   (R.(Simulation.Definitions.compile) rec2)
+  (R.(Simulation.Definitions.compile) rec2)  ret' /\
+  length lo = length lo') -> 
+
+(forall o s s' grs1 l_grs1', 
+exec L1 u o s (R.(Simulation.Definitions.compile) rec2) (Crashed s') ->
+(exists sa, refines_reboot s sa) ->
+l_grs1 = grs1::l_grs1' ->
+exists sa', refines_reboot (grs1 s') sa') ->
+
+abstract_oracles_exist_wrt HCR XXXXX u
+  rec rec l_grs2.
+Proof.
+    unfold abstract_oracles_exist_wrt; simpl; 
+    induction l_grs1; simpl; intros;
+    eapply_fresh forall2_length in H1;
+    destruct l_grs2; simpl in *; try lia;
+    unfold HC_refines in *; cleanup;
+    repeat invert_exec; cleanup.
+    {
+        rewrite H2 in H14.
+        eapply lift2_invert_exec in H14 ; cleanup.
+        simpl in *.
+        
+        edestruct H; eauto.
+        simpl; econstructor; eauto.
+
+        simpl in *; cleanup; try intuition;
+        cleanup; repeat unify_execs; cleanup.
+        exists ([(map
+        (fun o0 : Language.token' O2 =>
+         match o0 with
+         | OpToken _ o1 =>
+             OpToken (HorizontalComposition O O2)
+               (Token2 O O2 o1)
+         | Language.Crash _ =>
+             Language.Crash
+               (HorizontalComposition O O2)
+         | Language.Cont _ =>
+             Language.Cont
+               (HorizontalComposition O O2)
+         end) o)]).
+        simpl; split; eauto.
+        destruct si.
+        left; do 2 eexists; intuition eauto.
+        rewrite H2.
+        eapply lift2_exec_step; eauto.
+        eapply HC_oracle_refines_2; eauto.
+    }
+    {
+      inversion H1; cleanup.
+      rewrite H2 in H17.
+      eapply_fresh lift2_invert_exec_crashed in H17; cleanup.
+      simpl in *.
+
+      edestruct H3; eauto; cleanup.
+      edestruct H; eauto.
+      econstructor; eauto.
+      rewrite H10; eauto.
+      simpl in *; cleanup; try tauto.
+      split_ors; cleanup; repeat unify_execs; cleanup.
+
+      edestruct H0; eauto.
+      rewrite H10; eauto.
+      simpl in *; cleanup; try tauto.
+
+      simpl in *; eexists (_::_); simpl.
+      split; eauto.
+      setoid_rewrite H11; eauto.
+      rewrite map_length.
+      apply H13.
+      
+      right.
+      eexists; intuition eauto.
+      rewrite H2; simpl; eauto.
+*)
+
+
+(*
+Lemma HC_abstract_oracles_exist_wrt_2:
+forall O O1 O2
+(L1: Language O1) (L2: Language O2)
+(HCL1: Language (HorizontalComposition O O1))
+(HCL2: Language (HorizontalComposition O O2))
+(RC: CoreRefinement L1 O2)
+(l_grs1: list (L1.(state) -> L1.(state))) 
+(l_grs2: list (HCL1.(state) -> HCL1.(state)))
+u T (p: L2.(prog) T) 
+(rec: HCL2.(prog) unit) 
+(rec2: L2.(prog) unit)
+refines_reboot,
+
+let R := LiftRefinement L2 RC in
+let HCR := HC_Refinement HCL1 HCL2 RC in
+
+abstract_oracles_exist_wrt R R.(refines) u p rec2 l_grs1 ->
+(forall grs1 l_grs1', 
+l_grs1 = grs1::l_grs1' ->
+abstract_oracles_exist_wrt R refines_reboot u rec2 rec2 l_grs1') ->
+Forall2 (fun f1 f2 => forall (s: (O.(Core.state) * L1.(state))), f1 (snd s) = snd (f2 s)) l_grs1 l_grs2 ->
+(forall T (p: L2.(prog) T), HCR.(Simulation.Definitions.compile) (lift_L2 _ p) = lift_L2 _ (R.(Simulation.Definitions.compile) p)) ->
+
+(forall lo s ret grs1 grs2 l_grs1' l_grs2', 
+recovery_exec' u lo s l_grs2'
+(HCR.(Simulation.Definitions.compile) rec)
+(HCR.(Simulation.Definitions.compile) rec) ret ->
+l_grs1 = grs1::l_grs1' ->
+l_grs2 = grs2::l_grs2' ->
+exists lo' ret',
+   recovery_exec' u lo' (snd s) l_grs1' 
+   (R.(Simulation.Definitions.compile) rec2)
+  (R.(Simulation.Definitions.compile) rec2)  ret' /\
+  length lo = length lo') -> 
+
+(forall o s s' grs1 l_grs1', 
+exec L1 u o s (R.(Simulation.Definitions.compile) p) (Crashed s') ->
+(exists sa, R.(refines) s sa) ->
+l_grs1 = grs1::l_grs1' ->
+exists sa', refines_reboot (grs1 s') sa') ->
+
+(forall u s T (op:O2.(operation) T) o t, 
+token_refines RC u s op (fun s1 : state L1 => s1) o t ->
+minimal_oracle (compile_core RC op) u s o) ->
+
+abstract_oracles_exist_wrt HCR HCR.(refines) u
+  (lift_L2 _ p) rec l_grs2.
+Proof.
+    unfold abstract_oracles_exist_wrt; simpl; 
+    induction l_grs1; simpl; intros;
+    eapply_fresh forall2_length in H1;
+    destruct l_grs2; simpl in *; try lia;
+    unfold HC_refines in *; cleanup;
+    repeat invert_exec; cleanup.
+    {
+        rewrite H2 in H15.
+        eapply lift2_invert_exec in H15 ; cleanup.
+        simpl in *.
+        
+        edestruct H; eauto.
+        simpl; econstructor; eauto.
+
+        simpl in *; cleanup; try intuition;
+        cleanup; repeat unify_execs; cleanup.
+        exists ([(map
+        (fun o0 : Language.token' O2 =>
+         match o0 with
+         | OpToken _ o1 =>
+             OpToken (HorizontalComposition O O2)
+               (Token2 O O2 o1)
+         | Language.Crash _ =>
+             Language.Crash
+               (HorizontalComposition O O2)
+         | Language.Cont _ =>
+             Language.Cont
+               (HorizontalComposition O O2)
+         end) o)]).
+        simpl; split; eauto.
+        destruct si.
+        left; do 2 eexists; intuition eauto.
+        rewrite H2.
+        eapply lift2_exec_step; eauto.
+        eapply HC_oracle_refines_2; eauto.
+    }
+    {
+      inversion H1; cleanup.
+      rewrite H2 in H18.
+      eapply_fresh lift2_invert_exec_crashed in H18; cleanup.
+      simpl in *.
+
+      edestruct H3; eauto; cleanup.
+      edestruct H; eauto.
+      econstructor; eauto.
+      rewrite H11; eauto.
+      simpl in *; cleanup; try tauto.
+      split_ors; cleanup; repeat unify_execs; cleanup.
+
+      edestruct H0; eauto.
+      rewrite H11; eauto.
+      simpl in *; cleanup; try tauto.
+
+      simpl in *; eexists (_::_); simpl.
+      split; eauto.
+      setoid_rewrite H12; eauto.
+      rewrite map_length.
+      apply H14.
+      
+      right.
+      eexists; intuition eauto.
+      rewrite H2; simpl; eauto.
+
+      unfold oracle_refines.
+      
+      admit.
+      
+
+      admit.
+    }
+Abort.
+*)
+
+Require Import TransactionalDiskRefinement.
+
+Lemma AOE_recover:
+forall n u,
+abstract_oracles_exist_wrt
+(LiftRefinement AuthenticatedDisk
+  (HC_Core_Refinement ATCLang AuthenticatedDisk
+  Definitions.TransactionalDiskCoreRefinement))
+(fun s1 s2 => refines_reboot (snd s1) (snd s2))
+u
+recover
+recover (ATC_reboot_list n).
+Proof.
+    unfold ATC_reboot_list,
+    abstract_oracles_exist_wrt;
+    induction n; simpl; intros.
+    { (* base case *)
+      repeat invert_exec; cleanup.
+      eapply_fresh minimal_oracle_finished_same in H7.
+      invert_exec'' H7.
+      invert_exec'' H6.
+      repeat invert_exec; cleanup.
+      invert_exec'' H10.
+      invert_exec'' H6.
+      repeat invert_exec; cleanup.
+      eexists [_]; simpl.
+      intuition eauto.
+      left; intuition eauto.
+      do 2 eexists; intuition eauto.
+      repeat (rewrite cons_app;
+      repeat econstructor; eauto).
+      eexists; intuition eauto.
+      do 4 eexists; intuition eauto.
+      simpl; eexists; intuition eauto.
+      simpl; eexists; intuition eauto.
+      left; do 2 eexists; intuition eauto.
+      repeat (rewrite cons_app;
+      repeat econstructor; eauto).
+    }
+    { (* Inductive case *)
+      repeat invert_exec; cleanup.
+      eapply_fresh exec_crashed_minimal_oracle in H10; cleanup.
+      invert_exec'' H10; repeat invert_exec; cleanup.
+      {
+        invert_exec'' H8; repeat invert_exec; cleanup.
+        invert_exec'' H13; repeat invert_exec; cleanup.
+        edestruct IHn; only 2: eauto.
+        simpl; unfold refines, HC_refines,
+        refines_reboot in *; simpl in *;
+        unfold TransactionToTransactionalDisk.Definitions.refines,
+        Transaction.transaction_reboot_rep in *; 
+        simpl in *; cleanup.
+        eexists; eauto.
+        split_ors; cleanup; repeat invert_exec.
+      rewrite <- app_assoc in H0; simpl in *; cleanup.
+
+      Lemma crashed_extend_oracle:
+      forall O (L: Language O) T (p: L.(prog) T) u s o o' s',
+      exec L u o s p (Crashed s') ->
+      exec L u (o++o') s p (Crashed s').
+      Proof.
+        induction p; intros; repeat invert_exec.
+        econstructor.
+
+      eexists (_::_); 
+      simpl; intuition eauto.
+      eapply recovery_oracles_refine_to_length in H1.
+      rewrite H1; eauto.
+      eauto.
+      
+      right; intuition eauto.
+      eexists; intuition eauto.
+      rewrite cons_app.
+      repeat econstructor.
+      Search Crashed.
+      eapply ExecOpCrash.
+      simpl.
+
+            eapply ExecP2Crash with (s:= (fst si, ([], snd (snd si)))).
+      repeat econstructor; eauto.
+      eexists; intuition eauto.
+      do 3 eexists; intuition eauto.
+      simpl.
+      do 2 eexists; intuition eauto.
+      rewrite app_nil_r; eauto.
+      simpl; intuition eauto.
+      do 2 eexists; intuition eauto.
+      {
+        unfold minimal_oracle; intros.
+        intros Hn; simpl in *.
+        destruct n0; simpl in *.
+        eapply exec_empty_oracle; eauto.
+        destruct n0; simpl in *; try lia.
+        invert_exec'' Hn.
+        apply app_eq_unit in H3;
+        split_ors; cleanup; 
+        eapply exec_empty_oracle; eauto.
+        apply app_eq_unit in H3;
+        split_ors; cleanup; 
+        try solve [eapply exec_empty_oracle; eauto].
+        invert_exec'' H8; repeat invert_exec.
+      }
+
+      right. do 2 eexists.
+      unfold Transaction.recover.
+      rewrite cons_app;
+      econstructor; eauto.
+      repeat econstructor; eauto.
+      repeat econstructor; eauto.
+      intuition eauto.
+    }
+    {
+      (* eapply exec_crashed_minimum_oracle in H5; cleanup. 
+      rewrite <- app_assoc. *)
+      invert_exec'' H5; repeat invert_exec; cleanup.
+      edestruct IHn; only 2: eauto.
+      simpl; unfold refines, HC_refines,
+      refines_reboot in *; simpl in *;
+      unfold TransactionToTransactionalDisk.Definitions.refines,
+      Transaction.transaction_reboot_rep in *; 
+      simpl in *; cleanup.
+      eexists; eauto.
+
+      eexists (_::_); 
+      simpl; intuition eauto.
+      eapply recovery_oracles_refine_to_length in H0.
+      rewrite H0; eauto.
+      eauto.
+      
+      right; intuition eauto.
+      eexists; intuition eauto.
+      rewrite cons_app;
+      eapply ExecBindCrash.
+      repeat econstructor; eauto.
+      eexists; intuition eauto.
+      do 3 eexists; intuition eauto.
+      do 2 eexists; intuition eauto.
+      instantiate (1:= o2).
+      rewrite cons_app; eauto.
+      simpl; eauto.
+      {
+        unfold minimal_oracle; intros.
+        intros Hn; simpl in *.
+        destruct n0; simpl in *; try lia.
+        eapply exec_empty_oracle; eauto.
+      }
+      right; do 2 eexists; intuition eauto.
+      unfold Transaction.recover.
+      rewrite cons_app;
+      eapply ExecBindCrash; eauto.
+      repeat econstructor; eauto.
+      destruct si.
+      simpl.
+      destruct s0.
+      repeat econstructor; eauto.
+    }
+  }
+  Unshelve.
+  all: exact TransactionCacheLang.
+  Qed.
+
+
+  Lemma compile_lift2_comm:
+  forall u T (p: TransactionalDisk.(prog) T) o s ret,
+  Language.exec' u o s
+  (RefinementLift.compile
+      (HorizontalComposition AuthenticationOperation
+        TransactionCacheOperation)
+      (HorizontalComposition AuthenticationOperation
+        (TransactionalDiskLayer.TransactionalDiskOperation
+            FSParameters.data_length)) ATCLang AuthenticatedDisk
+      (HC_Core_Refinement ATCLang AuthenticatedDisk
+        TransactionalDiskCoreRefinement) T
+      (lift_L2 AuthenticationOperation p)) ret ->
+
+      Language.exec' u o s
+      (lift_L2 AuthenticationOperation 
+        (TransactionalDiskRefinement.(Simulation.Definitions.compile) p)) ret.
+  Proof.
+    induction p; simpl; intros; eauto.
+    invert_exec'' H0.
+    eapply IHp in H7.
+    eapply H in H10.
+    econstructor; eauto.
+    eapply IHp in H6.
+    eapply ExecBindCrash; eauto.
+  Qed.
+
+
+  Lemma compile_lift2_comm_rev:
+  forall u T (p: TransactionalDisk.(prog) T) o s ret,
+  Language.exec' u o s
+      (lift_L2 AuthenticationOperation 
+        (TransactionalDiskRefinement.(Simulation.Definitions.compile) p)) ret ->
+  
+  Language.exec' u o s
+  (RefinementLift.compile
+      (HorizontalComposition AuthenticationOperation
+        TransactionCacheOperation)
+      (HorizontalComposition AuthenticationOperation
+        (TransactionalDiskLayer.TransactionalDiskOperation
+            FSParameters.data_length)) ATCLang AuthenticatedDisk
+      (HC_Core_Refinement ATCLang AuthenticatedDisk
+        TransactionalDiskCoreRefinement) T
+      (lift_L2 AuthenticationOperation p)) ret.
+  Proof.
+    induction p; simpl; intros; eauto.
+    invert_exec'' H0.
+    eapply IHp in H7.
+    eapply H in H10.
+    econstructor; eauto.
+    eapply IHp in H6.
+    eapply ExecBindCrash; eauto.
+  Qed.
+
+
+
+Lemma ATC_AOE:
+forall u T (p: TransactionalDisk.(prog) T) n, 
+
+(forall o s s' r, 
+(exists s1, ATC_Refinement.(Simulation.Definitions.refines) s s1) ->
+exec TransactionCacheLang u o (snd s) 
+(TransactionalDiskRefinement.(Simulation.Definitions.compile) p) (Finished s' r) ->
+exists oa, oracle_refines _ _
+  ATCLang AuthenticatedDisk
+  ATC_CoreRefinement T u s
+  (lift_L2 AuthenticationOperation p)
+  (fun
+     s : HorizontalComposition.state'
+           AuthenticationOperation
+           TransactionCacheOperation
+   => s) (map
+       (fun o : Language.token' TransactionCacheOperation =>
+        match o with
+        | OpToken _ o1 =>
+            OpToken
+              (HorizontalComposition AuthenticationOperation
+                 TransactionCacheOperation)
+              (Token2 AuthenticationOperation
+                 TransactionCacheOperation o1)
+        | Language.Crash _ =>
+            Language.Crash
+              (HorizontalComposition AuthenticationOperation
+                 TransactionCacheOperation)
+        | Language.Cont _ =>
+            Language.Cont
+              (HorizontalComposition AuthenticationOperation
+                 TransactionCacheOperation)
+        end) o) oa) ->
+
+        (forall o s s', 
+(exists s1, ATC_Refinement.(Simulation.Definitions.refines) s s1) ->
+Language.exec' u o s
+        (RefinementLift.compile
+           (HorizontalComposition AuthenticationOperation
+              TransactionCacheOperation)
+           (HorizontalComposition AuthenticationOperation
+              (TransactionalDiskLayer.TransactionalDiskOperation
+                 FSParameters.data_length)) ATCLang AuthenticatedDisk
+           (HC_Core_Refinement ATCLang AuthenticatedDisk
+              TransactionalDiskCoreRefinement) T
+           (lift_L2 AuthenticationOperation p)) (Crashed s') ->
+exists oa, oracle_refines _ _
+  ATCLang AuthenticatedDisk
+  ATC_CoreRefinement T u s
+  (lift_L2 AuthenticationOperation p)
+  (fun
+     s : HorizontalComposition.state'
+           AuthenticationOperation
+           TransactionCacheOperation
+   => (fst s, ([], snd (snd s)))) o oa) ->
+
+(forall o s s', 
+(exists s1, refines s s1) ->
+exec TransactionCacheLang u o s 
+(TransactionalDiskRefinement.(Simulation.Definitions.compile) p) (Crashed s') ->
+exists s1', refines_reboot s' s1') ->
+abstract_oracles_exist_wrt ATC_Refinement
+  (ATC_Refinement.(Simulation.Definitions.refines)) u
+  (@lift_L2 AuthenticationOperation _ TransactionalDisk _ p) 
+  File.recover (ATC_reboot_list n).
+Proof.
+    intros; destruct n; simpl; eauto.
+    {
+      unfold abstract_oracles_exist_wrt, ATC_reboot_list in *; 
+      simpl in *; intros.
+      repeat invert_exec.
+      eapply_fresh compile_lift2_comm in H10.
+      eapply lift2_invert_exec in Hx; cleanup.
+      edestruct H; eauto.
+
+      eexists [_]; simpl; eauto.
+      split; intuition eauto.
+      left; do 2 eexists; intuition eauto.
+    }
+    {
+      unfold abstract_oracles_exist_wrt, ATC_reboot_list in *; 
+      simpl in *; intros.
+      repeat invert_exec.
+      edestruct AOE_recover; eauto.
+      {
+        unfold HC_refines in *; 
+        simpl in *; cleanup.
+        eapply compile_lift2_comm in H13.
+        eapply lift2_invert_exec_crashed in H13; cleanup.
+        edestruct H1; eauto.
+        unfold refines_reboot, Transaction.transaction_reboot_rep in *; 
+        simpl in *; eauto.
+        exists (fst x, (snd x2, snd x2)); eauto.
+      }
+
+      eapply_fresh compile_lift2_comm in H13.
+      eapply lift2_invert_exec_crashed in Hx; cleanup.
+      edestruct H0; eauto.
+
+      eexists (_ :: _).
+      simpl.
+      intuition eauto.
+      eapply recovery_oracles_refine_to_length in H3; eauto.
+    }
+    Unshelve.
+    all: exact ATCLang.
+Qed.
