src/Noninterference/TransactionalDisk/Simulations/ATCSimulation.v
@@ -1,0 +1,723 @@
+Require Import Lia Framework FSParameters FileDiskLayer. (* LoggedDiskLayer TransactionCacheLayer TransactionalDiskLayer. *)
+Require Import FileDiskNoninterference FileDiskRefinement.
+Require Import ATCLayer TransferProofs.
+Require Import TransactionalDiskRefinement.
+Require Import Coq.Program.Equality.
+Require Import Eqdep.
+
+Set Nested Proofs Allowed.
+
+Fixpoint not_init {T} (p: AuthenticatedDisk.(prog) T) :=
+  match p with
+  | Op _ o =>
+    match o with
+    | P1 _ => True
+    | P2 o =>
+    (forall l, ~eq_dep Type (operation Definitions.abs_op) _ o 
+    unit (TransactionalDiskLayer.Init l))
+    end
+  | Ret _ => True
+  | Bind p1 p2 =>
+  not_init p1 /\ forall t, not_init (p2 t)
+  end.
+
+
+Lemma HC_exec_same_finished:
+  forall u T (p: AuthenticatedDisk.(prog) T) 
+  o o0 s_imp s_abs x x0,
+  not_init p ->
+  Language.exec' u o s_imp
+ (ATC_Refinement.(Simulation.Definitions.compile) p)
+ (Finished x x0) ->
+
+ oracle_refines _ _ _ _ ATC_CoreRefinement T u s_imp
+ p
+ (fun s : HorizontalComposition.state'
+          AuthenticationOperation
+          TransactionCacheOperation => s) o o0 ->
+
+ ATC_Refinement.(Simulation.Definitions.refines) s_imp s_abs ->
+
+  (forall u s_imp s_abs T o x x0 x2 x3 x4,
+  exec Definitions.imp u x3 s_imp
+ (compile T o) (Finished x x0) ->
+ token_refines T u s_imp o x4 x3 x2 ->
+ refines s_imp s_abs ->
+ (forall l, ~eq_dep Type (operation Definitions.abs_op) T o unit (TransactionalDiskLayer.Init l)) ->
+exists s_abs',
+TransactionalDiskLayer.exec' data_length u x2
+  s_abs o (Finished s_abs' x0) /\
+refines x s_abs') ->
+ exists s_abs' : Recovery_Result,
+  recovery_exec AuthenticatedDisk u [o0] s_abs
+    (authenticated_disk_reboot_list 0) p
+    File.recover s_abs' /\
+    ATC_Refinement.(Simulation.Definitions.refines) x
+    (extract_state_r s_abs') /\
+  Some x0 = extract_ret_r s_abs'.
+Proof.
+  induction p; simpl; intros.
+  {
+    cleanup; simpl in *.
+    {
+      invert_exec'' H0.
+      invert_exec.
+      unfold HC_refines in *; simpl in *; cleanup.
+      unfold authenticated_disk_reboot_list; simpl.
+      eexists (RFinished _ _); split.
+      repeat econstructor; eauto.
+      simpl; intuition eauto.
+    }
+    {
+      eapply lift2_invert_exec in H0; cleanup.
+      (*apply HC_oracle_transformation_id in h; subst. *)
+      unfold HC_refines in *; simpl in *; cleanup.
+      unfold authenticated_disk_reboot_list; simpl.
+      eapply_fresh H3 in H4; eauto; cleanup.
+      eexists (RFinished _ _); split.
+      repeat econstructor; eauto.
+      simpl; intuition eauto.
+      eapply_fresh minimal_oracle_finished_same in H4.
+
+      Lemma minimal_oracle_prefix:
+      forall o1 o2 o3 o4 u s T (p: TransactionCacheLang.(prog) T) ret,
+      minimal_oracle p u s o4 ->
+      minimal_oracle p u s o3 ->
+      @HC_oracle_transformation _ _ TransactionCacheLang ATCLang o1 o4 ->
+      exec Definitions.imp u o3 s p ret ->
+      o1 ++ o2 = map (fun o : Language.token' TransactionCacheOperation =>
+      match o with
+      | OpToken _ o1 =>
+          OpToken
+            (HorizontalComposition AuthenticationOperation
+               TransactionCacheOperation)
+            (Token2 AuthenticationOperation TransactionCacheOperation o1)
+      | Language.Crash _ =>
+          Language.Crash
+            (HorizontalComposition AuthenticationOperation
+               TransactionCacheOperation)
+      | Language.Cont _ =>
+          Language.Cont
+            (HorizontalComposition AuthenticationOperation
+               TransactionCacheOperation)
+      end) o3 ->
+      o4 = o3.
+      Proof.
+        unfold minimal_oracle, HC_oracle_transformation; 
+        induction o1; simpl; intros; cleanup.
+        
+        subst,
+
+
+
+      (* Minimal oracle unique *)
+      admit.
+    }
+  }
+  {
+    cleanup; simpl in *.
+    split_ors; cleanup; repeat unify_execs; cleanup.
+    invert_exec'' H0.
+    unfold HC_refines in *; simpl in *; cleanup.
+    unfold authenticated_disk_reboot_list; simpl.
+    eexists (RFinished _ _); split.
+    repeat econstructor; eauto.
+    simpl; intuition eauto.
+  }
+  {
+    cleanup; simpl in *.
+    invert_exec'' H1.
+    split_ors; cleanup; simpl in *;
+    repeat unify_execs; cleanup.
+    {
+      exfalso; eapply finished_not_crashed_oracle_prefix; eauto.
+      eauto.
+    }
+    {
+      eapply exec_finished_deterministic_prefix in H1; eauto; cleanup.
+      repeat unify_execs; cleanup.
+
+      edestruct IHp; eauto.
+      cleanup; invert_exec; simpl in *; cleanup.
+      edestruct H; eauto.
+      cleanup; invert_exec; simpl in *; cleanup.
+      eexists (RFinished _ _); split; eauto.
+      repeat econstructor; eauto.
+      simpl; eauto.
+    }
+  }
+Admitted.
+
+
+Lemma HC_exec_same_crashed:
+  forall u T (p: AuthenticatedDisk.(prog) T) 
+  o o0 s_imp s_abs x,
+  not_init p ->
+  Language.exec' u o s_imp
+ (ATC_Refinement.(Simulation.Definitions.compile) p)
+ (Crashed x) ->
+
+ oracle_refines _ _ _ _ ATC_CoreRefinement T u s_imp
+ p
+ (fun s : HorizontalComposition.state'
+          AuthenticationOperation
+          TransactionCacheOperation => (fst s,
+          ([], snd (snd s)))) o o0 ->
+
+ ATC_Refinement.(Simulation.Definitions.refines) s_imp s_abs -> 
+
+  (forall u s_imp s_abs T o x x2 x3 x4 x5,
+
+      exec Definitions.imp u x3 s_imp
+    (compile T o) (Crashed x) ->
+    token_refines T u s_imp o x4 (x3 ++ x5) x2 ->
+    refines s_imp s_abs ->
+    (forall l, ~eq_dep Type (operation Definitions.abs_op) T o unit (TransactionalDiskLayer.Init l)) ->
+    exists s_abs',
+    TransactionalDiskLayer.exec' data_length u x2
+      s_abs o (Crashed s_abs') /\
+    refines_reboot x s_abs') ->
+
+    (forall u s_imp s_abs T o x x0 x2 x3 x4,
+    exec Definitions.imp u x3 s_imp
+   (compile T o) (Finished x x0) ->
+   token_refines T u s_imp o x4 x3 x2 ->
+   refines s_imp s_abs ->
+   (forall l, ~eq_dep Type (operation Definitions.abs_op) T o unit (TransactionalDiskLayer.Init l)) ->
+  exists s_abs',
+  TransactionalDiskLayer.exec' data_length u x2
+    s_abs o (Finished s_abs' x0) /\
+  refines x s_abs') ->
+
+  (forall T o2 u s_imp x x1 x2 x3 x4 x5 x6 x7,
+    @HC_oracle_transformation AuthenticationOperation _ TransactionCacheLang ATCLang x5 x4 ->
+    minimal_oracle (compile T o2) u s_imp x4 ->
+    token_refines T u s_imp o2 x7 x4 x3 ->
+    x5 ++ x6 =
+     map
+       (fun o : Language.token' TransactionCacheOperation =>
+        match o with
+        | OpToken _ o1 =>
+            OpToken
+              (HorizontalComposition AuthenticationOperation
+                 TransactionCacheOperation)
+              (Token2 AuthenticationOperation TransactionCacheOperation o1)
+        | Language.Crash _ =>
+            Language.Crash
+              (HorizontalComposition AuthenticationOperation
+                 TransactionCacheOperation)
+        | Language.Cont _ =>
+            Language.Cont
+              (HorizontalComposition AuthenticationOperation
+                 TransactionCacheOperation)
+        end) x2 ++ x1 ->
+        exec Definitions.imp u x2 s_imp (compile T o2) (Crashed x) ->
+    token_refines T u s_imp o2 x7 x2 x3) -> 
+
+ exists s_abs',
+ Language.exec' u o0 s_abs p (Crashed s_abs') /\
+  refines_reboot (snd x) (snd s_abs').
+Proof.
+  induction p; simpl; intros.
+  {
+    cleanup; simpl in *.
+    {
+      invert_exec'' H0.
+      invert_exec.
+      unfold HC_refines in *; simpl in *; cleanup.
+      eexists; split.
+      repeat econstructor; eauto.
+      simpl; intuition eauto.
+      unfold refines, refines_reboot,
+      Transaction.transaction_rep,
+      Transaction.transaction_reboot_rep in *;
+      cleanup; eauto.
+    }
+    {
+      eapply lift2_invert_exec_crashed in H0; cleanup.
+      unfold HC_refines in *; simpl in *; cleanup.
+      (* apply HC_oracle_transformation_id_crashed in H5; cleanup.  *)
+      unfold authenticated_disk_reboot_list; simpl.
+      eapply H3 in H6; eauto; cleanup.
+      eexists; split.
+      repeat econstructor; eauto.
+      simpl; intuition eauto.
+      rewrite app_nil_r; eauto.
+    }
+  }
+  {
+    cleanup; simpl in *.
+    split_ors; cleanup; repeat unify_execs; cleanup.
+    invert_exec'' H0.
+    unfold HC_refines in *; simpl in *; cleanup.
+    unfold authenticated_disk_reboot_list; simpl.
+    eexists; split.
+    repeat econstructor; eauto.
+    simpl; intuition eauto.
+    unfold refines, refines_reboot,
+      Transaction.transaction_rep,
+      Transaction.transaction_reboot_rep in *;
+      cleanup; eauto.
+  }
+  {
+    cleanup; simpl in *.
+    invert_exec'' H1.
+    split_ors; cleanup; simpl in *;
+    repeat unify_execs; cleanup.
+    {
+      exfalso; eapply finished_not_crashed_oracle_prefix; eauto.
+      eauto.
+    }
+    {
+      eapply exec_finished_deterministic_prefix in H1; eauto; cleanup.
+      repeat unify_execs; cleanup.
+
+      edestruct HC_exec_same_finished; eauto.
+      cleanup; invert_exec; simpl in *; cleanup.
+      edestruct H; eauto.
+      cleanup; simpl in *; cleanup.
+      eexists; split; eauto.
+      repeat econstructor; eauto.
+    }
+    {
+      split_ors; cleanup; simpl in *;
+      repeat unify_execs; cleanup.
+      {
+        eapply_fresh exec_deterministic_wrt_oracle_prefix in H1; eauto; cleanup.
+        edestruct IHp.
+        3: eauto.
+        eauto.
+        eauto.
+        all: eauto.
+        cleanup.
+        eexists; split; eauto.
+        solve [econstructor; eauto].
+      }
+      {
+        symmetry in H2; 
+        exfalso; eapply finished_not_crashed_oracle_prefix; eauto.
+        eauto.
+      }
+    }
+  }
+Qed.
+
+Theorem recover_simulation:
+forall u n,
+SimulationForProgramGeneral _ _ _ _ ATC_Refinement 
+u _
+  File.recover File.recover
+  (ATC_reboot_list n)
+  (authenticated_disk_reboot_list n)
+  (fun s1 s2 => snd (snd s1) = snd (snd s2))
+  ATC_Refinement.(Simulation.Definitions.refines).
+  Proof.
+      unfold File.recover, 
+      SimulationForProgram,
+      SimulationForProgramGeneral,
+      ATC_reboot_list; 
+      induction n; simpl in *; intros.
+      {
+          repeat invert_exec.
+          simpl in *; cleanup; try tauto.
+          destruct l; simpl in *; try lia.
+          split_ors; cleanup; repeat unify_execs; cleanup.
+          invert_exec'' H8; repeat invert_exec.
+          invert_exec'' H11; repeat invert_exec.
+          invert_exec'' H14; repeat invert_exec.
+          simpl in *; cleanup.
+          inversion H; inversion H2; subst.
+          unfold HC_refines in *; simpl in *;
+          split_ors; cleanup.
+          {
+            edestruct recovery_simulation with (n:= 0); simpl.
+            3: unfold transaction_cache_reboot_list; 
+            simpl; econstructor; eauto.
+            instantiate (1:= [_]).
+            simpl; split; intuition eauto.
+            left; intuition eauto.
+             do 2 eexists; intuition eauto.
+             eexists; intuition eauto.
+
+             left; do 2 eexists; intuition eauto.
+             rewrite H0; eauto.
+
+             unfold refines, refines_reboot, Transaction.transaction_rep,
+             Transaction.transaction_reboot_rep in *.
+             cleanup; eauto.
+
+             cleanup.
+             unfold transactional_disk_reboot_list,
+             authenticated_disk_reboot_list in *; simpl in *; invert_exec.
+             simpl in *; cleanup; 
+             invert_exec'' H14; repeat invert_exec.
+             
+             eexists (RFinished _ _); split.
+             repeat (econstructor; eauto).
+             simpl; intuition eauto.
+             destruct s_imp; destruct s_abs; simpl.
+             destruct s, s1; eauto.
+             (*
+             unfold refines, Transaction.transaction_rep  in *; 
+             simpl in *; cleanup; eauto.
+             destruct t; eauto.
+             *)
+          }
+          {
+            unfold Transaction.recover in *; repeat invert_exec.
+            split_ors; cleanup; repeat invert_exec;
+            simpl in *; cleanup.
+            eexists; intuition eauto.
+            unfold authenticated_disk_reboot_list; simpl.
+            .
+          }
+      }
+      {
+        repeat invert_exec.
+          simpl in *; cleanup; try tauto.
+          split_ors; cleanup; repeat unify_execs; cleanup.
+          invert_exec'' H11; repeat invert_exec.
+          {
+            invert_exec'' H10; repeat invert_exec.
+            invert_exec'' H15; repeat invert_exec.
+            simpl in *; cleanup.
+            inversion H1; inversion H4; subst.
+            unfold HC_refines in *; simpl in *;
+            split_ors; cleanup.
+            {
+              unfold Transaction.recover in *; repeat invert_exec.
+              simpl in *; cleanup.
+            }
+            {
+              edestruct IHn; eauto.
+              instantiate (1:= (_, (_, _))); simpl; intuition eauto.
+
+              exists (Recovered (extract_state_r x0)).
+              simpl; intuition eauto.
+              
+              repeat econstructor; eauto.
+            }
+          }
+          {
+            invert_exec'' H9; repeat invert_exec.
+            simpl in *; cleanup.
+            inversion H1; subst.
+            unfold HC_refines in *; simpl in *;
+            split_ors; cleanup.
+            {
+              unfold Transaction.recover in *; repeat invert_exec.
+              simpl in *; cleanup.
+            }
+            {
+              edestruct IHn; eauto.
+              instantiate (1:= (_, (_, _))); simpl; intuition eauto.
+
+              exists (Recovered (extract_state_r x1)).
+              simpl; intuition eauto.
+              
+              repeat econstructor; eauto.
+            }
+          }
+      }
+  Qed.
+
+
+  Theorem HC_recovery_exec_same:
+      forall u T (p: AuthenticatedDisk.(prog) T) n 
+      l_o_imp l_o_abs s_imp s_abs s_imp',
+    not_init p ->
+      recovery_exec ATCLang u l_o_imp s_imp (ATC_reboot_list n)
+      (Simulation.Definitions.compile ATC_Refinement p)
+      (Simulation.Definitions.compile ATC_Refinement File.recover) s_imp' ->
+
+      recovery_oracles_refine_to ATC_Refinement u
+      s_imp p File.recover (ATC_reboot_list n) l_o_imp l_o_abs ->
+
+      Simulation.Definitions.refines
+       ATC_Refinement s_imp
+       s_abs ->
+
+       (forall u s_imp s_abs T o x x0 x2 x3 x4,
+       exec Definitions.imp u x3 s_imp
+      (compile T o) (Finished x x0) ->
+      token_refines T u s_imp o x4 x3 x2 ->
+      refines s_imp s_abs ->
+      (forall l, ~eq_dep Type (operation Definitions.abs_op) T o unit (TransactionalDiskLayer.Init l)) ->
+     exists s_abs',
+     TransactionalDiskLayer.exec' data_length u x2
+       s_abs o (Finished s_abs' x0) /\
+     refines x s_abs') ->
+
+     (forall u s_imp s_abs T o x x2 x3 x4 x5,
+     exec Definitions.imp u x3 s_imp
+   (compile T o) (Crashed x) ->
+   token_refines T u s_imp o x4 (x3 ++ x5) x2 ->
+   refines s_imp s_abs ->
+   (forall l, ~eq_dep Type (operation Definitions.abs_op) T o unit (TransactionalDiskLayer.Init l)) ->
+   exists s_abs',
+   TransactionalDiskLayer.exec' data_length u x2
+     s_abs o (Crashed s_abs') /\
+   refines_reboot x s_abs') ->
+
+      exists s_abs' : Recovery_Result,
+      recovery_exec AuthenticatedDisk u l_o_abs s_abs
+      (authenticated_disk_reboot_list n) p File.recover s_abs' /\
+      Simulation.Definitions.refines ATC_Refinement (extract_state_r s_imp')
+    (extract_state_r s_abs') /\ extract_ret_r s_imp' = extract_ret_r s_abs'.
+    Proof.
+      intros; destruct n.
+      {
+        invert_exec.
+        simpl in *; cleanup; try tauto.
+        destruct l; simpl in *; try lia.
+        split_ors; cleanup; repeat unify_execs; cleanup.
+        eapply HC_exec_same_finished; eauto.
+      }
+      {
+        unfold ATC_reboot_list in *; invert_exec.
+        simpl in *; cleanup; try tauto.
+        split_ors; cleanup; repeat unify_execs; cleanup.
+        simpl in *.
+        edestruct HC_exec_same_crashed; eauto; cleanup.
+        edestruct recover_simulation.
+        2: {
+          simpl in *;
+          instantiate (1:= (fst x0, (snd (snd x0), snd (snd x0)))); 
+          instantiate (1:= (fst x, ([], snd (snd x)))); 
+          simpl; intuition eauto.
+        }
+        all: eauto.
+        {
+          cleanup.
+          simpl in *; cleanup.
+          eexists (Recovered _); split.
+          unfold authenticated_disk_reboot_list; simpl; 
+          econstructor; eauto.
+          unfold HC_refines in *; simpl in *; cleanup.
+          simpl; split; eauto.
+        }
+      }
+Qed.
+
+
+Lemma operation_simulation_finished:
+      forall (u0 : user) (s_imp0 : Language.state' TransactionCacheOperation)
+      (s_abs0 : total_mem * total_mem) (T0 : Type)
+      (o : operation Definitions.abs_op T0)
+      (x : Language.state' TransactionCacheOperation) 
+      (x0 : T0) (x2 : TransactionalDiskLayer.token')
+      (x3 : oracle' TransactionCacheOperation)
+      (x4 : state Definitions.imp -> state Definitions.imp),
+    exec Definitions.imp u0 x3 s_imp0 (compile T0 o) (Finished x x0) ->
+    token_refines T0 u0 s_imp0 o x4 x3 x2 ->
+    refines s_imp0 s_abs0 ->
+    (forall l, ~eq_dep Type (operation Definitions.abs_op) T0 o unit (TransactionalDiskLayer.Init l)) ->
+    exists s_abs' : TransactionalDiskLayer.state',
+      TransactionalDiskLayer.exec' data_length u0 x2 s_abs0 o
+        (Finished s_abs' x0) /\ refines x s_abs'.
+    Proof.
+      intros; destruct o.
+      {
+        edestruct read_simulation with (n:= 0); eauto.
+        2: {
+          instantiate (1:= RFinished _ _).
+          eapply ExecFinished; eauto.
+          simpl in *; eauto.
+         }
+         instantiate (1:= [ _ ]). 
+         simpl; eauto.
+         split; eauto.
+         left; do 2 eexists; intuition eauto.
+         cleanup; simpl in *.
+         repeat invert_exec; simpl in *; cleanup.
+        invert_exec'' H12.
+         eexists; split; eauto.
+      }
+      {
+        edestruct write_simulation with (n:= 0); eauto.
+        2: {
+          instantiate (1:= RFinished _ _).
+          eapply ExecFinished; eauto.
+          simpl in *; eauto.
+         }
+         instantiate (1:= [ _ ]). 
+         simpl; eauto.
+         split; eauto.
+         left; do 2 eexists; intuition eauto.
+         cleanup; simpl in *.
+         repeat invert_exec; simpl in *; cleanup.
+        invert_exec'' H12.
+         eexists; split; eauto.
+      }
+      {
+        edestruct commit_simulation with (n:= 0); eauto.
+        2: {
+          instantiate (1:= RFinished _ _).
+          eapply ExecFinished; eauto.
+         }
+         instantiate (1:= [ _ ]). 
+         simpl; eauto.
+         split; eauto.
+         left; do 2 eexists; intuition eauto.
+         cleanup; simpl in *.
+         repeat invert_exec; simpl in *; cleanup.
+        invert_exec'' H12.
+         eexists; split; eauto.
+      }
+      {
+        edestruct abort_simulation with (n:= 0); eauto.
+        2: {
+          instantiate (1:= RFinished _ _).
+          eapply ExecFinished; eauto.
+         }
+         instantiate (1:= [ _ ]). 
+         simpl; eauto.
+         split; eauto.
+         left; do 2 eexists; intuition eauto.
+         cleanup; simpl in *.
+         repeat invert_exec; simpl in *; cleanup.
+        invert_exec'' H12.
+         eexists; split; eauto.
+      }
+      {
+        edestruct TransactionToTransactionalDisk.Refinement.recovery_simulation with (n:= 0); eauto.
+        3: {
+          instantiate (1:= RFinished _ _).
+          eapply ExecFinished; eauto.
+         }
+         instantiate (1:= [ _ ]). 
+         simpl; eauto.
+         split; eauto.
+         left; do 2 eexists; intuition eauto.
+         unfold refines, refines_reboot,
+         Transaction.transaction_rep,
+         Transaction.transaction_reboot_rep in *; 
+         cleanup; eauto.
+         cleanup; simpl in *.
+         repeat invert_exec; simpl in *; cleanup.
+        invert_exec'' H12.
+         eexists; split; eauto.
+      }
+      {
+        exfalso.
+        eapply H2.
+        eauto.
+      }
+    Qed.
+
+Lemma operation_simulation_crashed:
+    forall (u0 : user) (s_imp0 : Language.state' TransactionCacheOperation)
+  (s_abs0 : total_mem * total_mem) (T0 : Type)
+  (o : operation Definitions.abs_op T0)
+  (x : Language.state' TransactionCacheOperation)
+  (x2 : TransactionalDiskLayer.token')
+  (x3 : oracle' TransactionCacheOperation)
+  (x4 : state Definitions.imp -> state Definitions.imp)
+  (x5 : list (Language.token' TransactionCacheOperation)),
+exec Definitions.imp u0 x3 s_imp0 (compile T0 o) (Crashed x) ->
+token_refines T0 u0 s_imp0 o x4 (x3 ++ x5) x2 ->
+refines s_imp0 s_abs0 ->
+(forall l, ~eq_dep Type (operation Definitions.abs_op) _ o unit (TransactionalDiskLayer.Init l)) ->
+exists s_abs' : TransactionalDiskLayer.state',
+  TransactionalDiskLayer.exec' data_length u0 x2 s_abs0 o
+    (Crashed s_abs') /\ refines_reboot x s_abs'.
+    Proof.
+      intros; destruct o; simpl in *.
+      {
+        intuition cleanup.
+        eapply exec_deterministic_wrt_oracle_prefix in H; eauto; cleanup.
+        rewrite <- app_assoc; eauto.
+        eapply exec_deterministic_wrt_oracle_prefix in H; eauto; cleanup.
+
+        eexists; intuition eauto.
+        repeat econstructor.
+        unfold refines, refines_reboot,
+        Transaction.transaction_rep,
+        Transaction.transaction_reboot_rep in *; cleanup; eauto.
+        rewrite <- app_assoc; eauto.
+      }
+      {
+        intuition cleanup.
+        eapply exec_deterministic_wrt_oracle_prefix in H; eauto; cleanup.
+        rewrite <- app_assoc; eauto.
+        eapply exec_deterministic_wrt_oracle_prefix in H; eauto; cleanup.
+
+        eexists; intuition eauto.
+        repeat econstructor.
+
+        unfold refines, refines_reboot,
+        Transaction.transaction_rep,
+        Transaction.transaction_reboot_rep in *; cleanup; eauto.
+        rewrite <- app_assoc; eauto.
+      }
+      {
+        intuition cleanup.
+        eapply exec_deterministic_wrt_oracle_prefix in H; eauto; cleanup.
+        rewrite <- app_assoc; eauto.
+        eapply exec_deterministic_wrt_oracle_prefix in H; eauto; cleanup.
+
+        split_ors; cleanup.
+
+        eexists; intuition eauto.
+        repeat econstructor.
+        unfold refines, refines_reboot,
+        Transaction.transaction_rep,
+        Transaction.transaction_reboot_rep in *; cleanup; eauto.
+
+        eexists; intuition eauto.
+        repeat econstructor.
+        unfold refines, refines_reboot,
+        Transaction.transaction_rep,
+        Transaction.transaction_reboot_rep in *; cleanup; eauto.
+
+        rewrite <- app_assoc; eauto.
+      }
+      {
+        intuition cleanup.
+        eapply exec_deterministic_wrt_oracle_prefix in H; eauto; cleanup.
+        rewrite <- app_assoc; eauto.
+        eapply exec_deterministic_wrt_oracle_prefix in H; eauto; cleanup.
+
+        eexists; intuition eauto.
+        repeat econstructor.
+        
+        unfold refines, refines_reboot,
+        Transaction.transaction_rep,
+        Transaction.transaction_reboot_rep in *; cleanup; eauto.
+        rewrite <- app_assoc; eauto.
+      }
+      {
+        intuition cleanup.
+        eapply exec_deterministic_wrt_oracle_prefix in H; eauto; cleanup.
+        rewrite <- app_assoc; eauto.
+        eapply exec_deterministic_wrt_oracle_prefix in H; eauto; cleanup.
+
+        eexists; intuition eauto.
+        repeat econstructor.
+
+        unfold refines, refines_reboot,
+        Transaction.transaction_rep,
+        Transaction.transaction_reboot_rep in *; cleanup; eauto.
+        rewrite <- app_assoc; eauto.
+      }
+      { exfalso; eapply H2; eauto. }
+    Unshelve.
+    all: eauto.
+    Qed.
+
+
+Theorem ATC_simulation:
+forall u n T (p: AuthenticatedDisk.(prog) T),
+not_init p ->
+SimulationForProgram ATC_Refinement u
+  p File.recover
+  (ATC_reboot_list n)
+  (authenticated_disk_reboot_list n).
+  Proof.
+    unfold SimulationForProgram,
+    SimulationForProgramGeneral; 
+    intros.
+    eapply HC_recovery_exec_same; eauto.
+    eapply operation_simulation_finished.
+    apply operation_simulation_crashed.
+  Qed.
