src/Noninterference/TransactionalDisk/TransferProofs.v
@@ -1,105 +1,230 @@
 Require Import Framework FSParameters FileDiskLayer. (* LoggedDiskLayer TransactionCacheLayer TransactionalDiskLayer. *)
-Require Import TransactionalDiskRefinement FileDisk.TransferProofs FileDiskNoninterference ATCLayer.
+Require Import FileDiskNoninterference FileDiskRefinement.
+Require Import ATCLayer TransferProofs ATCSimulation.
 
 (* Notation "'TransactionalDiskCore'" := (TransactionalDiskOperation data_length). *)
 
-Fixpoint horizontally_compose_valid_prog1 {O1 O2} (L1: Language O1) (L2: Language O2) (LL: Language (HorizontalComposition O1 O2)) {T} (p1: prog L1 T) :=
-         match p1 with
-         | @Op _ T' p => Op (HorizontalComposition O1 O2) (P1 p)
-         | @Ret _ T' t => Ret t
-         | @Bind _ T1 T2 p1 p2 =>
-           Bind (horizontally_compose_valid_prog1 L1 L2 LL p1)
-           (fun r => horizontally_compose_valid_prog1 L1 L2 LL (p2 r))
-         end.
-
-
-Fixpoint horizontally_compose_valid_prog2 {O1 O2} (L1: Language O1) (L2: Language O2) (LL: Language (HorizontalComposition O1 O2)) {T} (p2: prog L2 T) :=
-         match p2 with
-         | @Op _ T' p => (Op (HorizontalComposition O1 O2) (P2 p))
-         | @Ret _ T' t => (Ret t)
-         | @Bind _ T1 T2 p1 p2 =>
-         Bind (horizontally_compose_valid_prog2 L1 L2 LL p1)
-         (fun r => horizontally_compose_valid_prog2 L1 L2 LL (p2 r))
-       end.
-
-
-Lemma ss_hc_rev_p1:
-  forall O1 O2 (L1: Language O1) (L2: Language O2) (LL: Language (HorizontalComposition O1 O2))
-    u R C V T l_grs1 l_grs2 (p1 p2: L1.(prog) T) rec,
-    @SelfSimulation _ LL u _ (horizontally_compose_valid_prog1 L1 L2 LL p1)
-    (horizontally_compose_valid_prog1 L1 L2 LL p2)
-    (horizontally_compose_valid_prog1 L1 L2 LL rec) R V  C l_grs2 ->
-    forall s2,
-      SelfSimulation u p1 p2 rec
-        (fun s1 => R (s1, s2))
-        (fun s1 s1' =>  V (s1, s2) (s1', s2))
-        C
-        l_grs1.
-Proof. Admitted.
-
-
-Lemma ss_hc_rev_p2:
-  forall O1 O2 (L1: Language O1) (L2: Language O2) (LL: Language (HorizontalComposition O1 O2))
-    u R C V T l_grs1 l_grs2 (p1 p2: L2.(prog) T) rec,
-    @SelfSimulation _ LL u _ (horizontally_compose_valid_prog2 L1 L2 LL p1)
-    (horizontally_compose_valid_prog2 L1 L2 LL p2)
-    (horizontally_compose_valid_prog2 L1 L2 LL rec) R V  C l_grs2 ->
-    forall s1,
-      SelfSimulation u p1 p2 rec
-        (fun s2 => R (s1, s2))
-        (fun s2 s2' =>  V (s1, s2) (s1, s2'))
-        C
-        l_grs1.
-Proof. Admitted.
-
-
-(*
-Theorem ss_TD_read:
-  forall n a u u' s,
-    @SelfSimulation _ TransactionalDisk u _
-    (TransactionalDiskCore.(Op) (Read a))
-    (TransactionalDiskCore.(Op) (Read a)) 
-    (TransactionalDiskCore.(Op) Recover) (TD_valid_state s) 
-    (TD_related_states u' None s) (eq u') (transactional_disk_reboot_list n).
-Proof.
-    intros.
-    eapply ss_hc_rev_p2 with (R:= AD_valid_state) (V:= AD_related_states u' None).
-    simpl; 
-    - apply ss_FD_read.
-    - apply read_simulation.
-    - apply read_simulation.
-    - apply abstract_oracles_exist_wrt_read.
-    - apply abstract_oracles_exist_wrt_read.
-    - apply ORS_read.
-    - unfold exec_compiled_preserves_validity,
-    refines_valid, FD_valid_state; intros; eauto.
-    - unfold exec_compiled_preserves_validity,
-    refines_valid, FD_valid_state; intros; eauto.
-    - unfold refines_related; apply SelfSimulation_Exists_read.
-Qed.
-*)
-
 Import FileDiskLayer.
+
+Theorem recovery_exec_termination_sensitive_bind:
+  forall O (L: Language O) 
+  T (p1 p2: L.(prog) T) 
+  T' (p3 p4: T -> L.(prog) T') rec s1 s2 
+  lob l_grs u s1',
+  (forall s1' lo lgrs, 
+  recovery_exec L u lo s1 lgrs p1 rec s1' ->
+   exists s2',
+   recovery_exec L u lo s2 lgrs p2 rec s2') ->
+
+  (forall s1' s2' s1r t1 t2 lo lo' lgrs, 
+  recovery_exec L u lo s1 [] p1 rec (RFinished s1' t1) ->
+  recovery_exec L u lo s2 [] p2 rec (RFinished s2' t2) ->
+    
+  recovery_exec L u lo' s1' lgrs (p3 t1) rec s1r ->
+  exists s2r,
+  recovery_exec L u lo' s2' lgrs (p4 t2) rec s2r) ->
+
+  recovery_exec L u lob s1 l_grs (Bind p1 p3) rec s1' ->
+   exists s2',
+   recovery_exec L u lob s2 l_grs (Bind p2 p4) rec s2'.
+Proof.
+  intros; repeat invert_exec.
+  {
+      invert_exec'' H10.
+
+      edestruct H.
+      econstructor; eauto.
+      invert_exec.
+
+      edestruct H0; eauto;
+      try solve [econstructor; eauto].
+      invert_exec.
+
+      eexists; repeat econstructor; eauto.
+  }
+  {
+    invert_exec'' H9.
+    {
+      edestruct H.
+      econstructor; eauto.
+      invert_exec.
+
+      edestruct H0; eauto;
+      try solve [econstructor; eauto].
+      invert_exec.
+
+      eexists; repeat econstructor; eauto.
+    }
+    {
+      edestruct H.
+      eapply ExecRecovered; eauto.
+      invert_exec.
+      eexists; eapply ExecRecovered; eauto.
+      eapply ExecBindCrash; eauto.
+    }
+  }
+Qed.
+  
+Lemma not_init_read:
+forall inum off,
+not_init (ATC_Refinement.(Simulation.Definitions.compile) (FileDisk.refinement.(Simulation.Definitions.compile) (FileDiskOp.(Op) (Read inum off)))).
+{
+        simpl.
+        Transparent Inode.get_owner.
+        unfold Inode.get_owner, Inode.get_inode,
+        Inode.InodeAllocator.read; simpl.
+        intuition eauto.
+        destruct (Compare_dec.lt_dec inum Inode.InodeAllocatorParams.num_of_blocks);
+        simpl; intuition eauto.
+        inversion H.
+        destruct (nth_error (value_to_bits t) inum);
+        simpl; intuition eauto.
+        destruct b; simpl; intuition eauto.
+        inversion H.
+        destruct t; simpl; intuition eauto.
+        destruct t; simpl; intuition eauto.
+        destruct t; simpl; intuition eauto.
+        destruct t; simpl; intuition eauto.
+        destruct u1; simpl; intuition eauto.
+        Transparent Inode.get_block_number.
+        unfold Inode.get_block_number,
+         Inode.get_inode, 
+         Inode.InodeAllocator.read ; simpl; intuition eauto.
+        destruct (Compare_dec.lt_dec inum Inode.InodeAllocatorParams.num_of_blocks);
+        simpl; intuition eauto.
+        inversion H.
+        destruct (nth_error (value_to_bits t) inum);
+        simpl; intuition eauto.
+        destruct b; simpl; intuition eauto.
+        inversion H.
+        destruct t; simpl; intuition eauto.
+        destruct t; simpl; intuition eauto.
+        destruct t; simpl; intuition eauto.
+        unfold File.DiskAllocator.read; simpl; intuition eauto.
+        destruct (Compare_dec.lt_dec a File.DiskAllocatorParams.num_of_blocks);
+        simpl; intuition eauto.
+        inversion H.
+        destruct (nth_error (value_to_bits t) a);
+        simpl; intuition eauto.
+        destruct b; simpl; intuition eauto.
+        inversion H.
+        destruct t; simpl; intuition eauto.
+        destruct t; simpl; intuition eauto.
+        all: inversion H.
+      }
+
 
 Theorem ss_ATC_read:
   forall n inum off u u',
     SelfSimulation u 
-    (compile (FileDisk.refinement.(Simulation.Definitions.compile) (FileDiskOp.(Op) (Read inum off)))) 
-    (compile (FileDisk.refinement.(Simulation.Definitions.compile) (FileDiskOp.(Op) (Read inum off)))) 
-    (compile (FileDisk.refinement.(Simulation.Definitions.compile) (FileDiskOp.(Op) Recover))) 
-    ATC_valid_state 
-    (ATC_related_states u' None) (eq u') (ATC_reboot_list n).
+    (ATC_Refinement.(Simulation.Definitions.compile) (FileDisk.refinement.(Simulation.Definitions.compile) (FileDiskOp.(Op) (Read inum off)))) 
+    (ATC_Refinement.(Simulation.Definitions.compile) (FileDisk.refinement.(Simulation.Definitions.compile) (FileDiskOp.(Op) (Read inum off)))) 
+    (ATC_Refinement.(Simulation.Definitions.compile) (FileDisk.refinement.(Simulation.Definitions.compile) (FileDiskOp.(Op) Recover))) 
+    (refines_valid ATC_Refinement AD_valid_state)
+    (refines_related ATC_Refinement (AD_related_states u' None))
+    (eq u') (ATC_reboot_list n).
 Proof.
-    intros; eapply SS_transfer.
-    - apply ss_FD_read.
-    - apply read_simulation.
-    - apply read_simulation.
-    - apply abstract_oracles_exist_wrt_read.
-    - apply abstract_oracles_exist_wrt_read.
-    - apply ORS_read.
-    - unfold exec_compiled_preserves_validity,
-    refines_valid, FD_valid_state; intros; eauto.
-    - unfold exec_compiled_preserves_validity,
-    refines_valid, FD_valid_state; intros; eauto.
-    - unfold refines_related; apply SelfSimulation_Exists_read.
-Qed.
+    intros. 
+    eapply SS_transfer.
+    - apply ss_AD_read.
+    - simpl. eapply ATC_simulation.
+      {
+        simpl.
+        Transparent Inode.get_owner.
+        unfold Inode.get_owner, Inode.get_inode,
+        Inode.InodeAllocator.read; simpl.
+        intuition eauto.
+        destruct (Compare_dec.lt_dec inum Inode.InodeAllocatorParams.num_of_blocks);
+        simpl; intuition eauto.
+        inversion H.
+        destruct (nth_error (value_to_bits t) inum);
+        simpl; intuition eauto.
+        destruct b; simpl; intuition eauto.
+        inversion H.
+        destruct t; simpl; intuition eauto.
+        destruct t; simpl; intuition eauto.
+        destruct t; simpl; intuition eauto.
+        destruct t; simpl; intuition eauto.
+        destruct u1; simpl; intuition eauto.
+        Transparent Inode.get_block_number.
+        unfold Inode.get_block_number,
+         Inode.get_inode, 
+         Inode.InodeAllocator.read ; simpl; intuition eauto.
+        destruct (Compare_dec.lt_dec inum Inode.InodeAllocatorParams.num_of_blocks);
+        simpl; intuition eauto.
+        inversion H.
+        destruct (nth_error (value_to_bits t) inum);
+        simpl; intuition eauto.
+        destruct b; simpl; intuition eauto.
+        inversion H.
+        destruct t; simpl; intuition eauto.
+        destruct t; simpl; intuition eauto.
+        destruct t; simpl; intuition eauto.
+        unfold File.DiskAllocator.read; simpl; intuition eauto.
+        destruct (Compare_dec.lt_dec a File.DiskAllocatorParams.num_of_blocks);
+        simpl; intuition eauto.
+        inversion H.
+        destruct (nth_error (value_to_bits t) a);
+        simpl; intuition eauto.
+        destruct b; simpl; intuition eauto.
+        inversion H.
+        destruct t; simpl; intuition eauto.
+        destruct t; simpl; intuition eauto.
+        all: inversion H.
+      }
+      - simpl. eapply ATC_simulation.
+      {
+        simpl.
+        Transparent Inode.get_owner.
+        unfold Inode.get_owner, Inode.get_inode,
+        Inode.InodeAllocator.read; simpl.
+        intuition eauto.
+        destruct (Compare_dec.lt_dec inum Inode.InodeAllocatorParams.num_of_blocks);
+        simpl; intuition eauto.
+        inversion H.
+        destruct (nth_error (value_to_bits t) inum);
+        simpl; intuition eauto.
+        destruct b; simpl; intuition eauto.
+        inversion H.
+        destruct t; simpl; intuition eauto.
+        destruct t; simpl; intuition eauto.
+        destruct t; simpl; intuition eauto.
+        destruct t; simpl; intuition eauto.
+        destruct u1; simpl; intuition eauto.
+        Transparent Inode.get_block_number.
+        unfold Inode.get_block_number,
+         Inode.get_inode, 
+         Inode.InodeAllocator.read ; simpl; intuition eauto.
+        destruct (Compare_dec.lt_dec inum Inode.InodeAllocatorParams.num_of_blocks);
+        simpl; intuition eauto.
+        inversion H.
+        destruct (nth_error (value_to_bits t) inum);
+        simpl; intuition eauto.
+        destruct b; simpl; intuition eauto.
+        inversion H.
+        destruct t; simpl; intuition eauto.
+        destruct t; simpl; intuition eauto.
+        destruct t; simpl; intuition eauto.
+        unfold File.DiskAllocator.read; simpl; intuition eauto.
+        destruct (Compare_dec.lt_dec a File.DiskAllocatorParams.num_of_blocks);
+        simpl; intuition eauto.
+        inversion H.
+        destruct (nth_error (value_to_bits t) a);
+        simpl; intuition eauto.
+        destruct b; simpl; intuition eauto.
+        inversion H.
+        destruct t; simpl; intuition eauto.
+        destruct t; simpl; intuition eauto.
+        all: inversion H.
+      }
+    - simpl. (* Use Lemmas *) admit.
+    - (* Use Lemmas *) admit.
+    - (* Use Lemmas *)admit.
+    - unfold exec_compiled_preserves_validity, AD_valid_state, 
+    refines_valid, FD_valid_state; 
+    intros; simpl; eauto.
+    - unfold exec_compiled_preserves_validity, AD_valid_state, 
+    refines_valid, FD_valid_state; 
+    intros; simpl; eauto.
+    - (* Use Lemmas *) admit.
+Abort.
